Modification on the proving process

Isabelle2/AbstractMultiPaxosR1.thy
@@ -1,82 +1,77 @@
 theory AbstractMultiPaxosR1
-imports  "../../IO-Automata/IOA" BallotArrays DistributedSafeAt
+imports  IOA BallotArrays DistributedSafeAt Paxos_Sig
 begin
 
-text {*
-1) Acceptors vote for a suggestion, and leaders use the distributed implementation of the safe-at computation.
-2) Explicit 1b messages.
-3) Explicit learning.
-4) Catch-up.
-5) Localizing suggestions (the leader function).
-6) Explicit leadership acquisition.
-*}
-
-type_synonym bal = nat
-type_synonym inst = nat
-text {* TODO: how to use real types, and the transfer package? *}
-
-record ('v,'a,'l) amp_state =
+record ('v,'a,'l) ampr1_state =
   propCmd :: "'v set"
   ballot :: "'a \<Rightarrow> bal"
   vote :: "'a \<Rightarrow> inst \<Rightarrow> bal \<rightharpoonup> 'v"
   suggestion :: "inst \<Rightarrow> bal \<rightharpoonup> 'v"
-  onebs :: "'a \<Rightarrow> bal \<rightharpoonup> (inst \<rightharpoonup> ('v \<times> bal))"
-  learned :: "'l \<Rightarrow> inst \<rightharpoonup> 'v"
-  leader :: "'a \<Rightarrow> bool"
+  onebs :: "'a \<Rightarrow> bal \<rightharpoonup> (inst \<Rightarrow> ('v\<times>bal) set)"
+  inst_status :: "bal \<rightharpoonup> inst \<rightharpoonup> 'v"
+  -- {* if @{term "inst_status s b = Some m"}, them @{term "m i = None"} means that 
+  all values are safe, and @{term "m i = Some v"} means that only @{term v} is known safe. *}
 
-locale amp_ioa = IOA +
-  fixes quorums::"'a set set" and leading :: "bal \<Rightarrow> 'a"
+locale ampr1_ioa =
+  fixes quorums::"'a set set" and leader :: "bal \<Rightarrow> 'a"
   -- {* @{term leader} determines the leader of a ballot. *}
 begin
 
-datatype ('vv,'aa,'ll) amp_action =
-  Propose 'vv
-| Learn nat 'vv 'll
-| Internal
+sublocale dsa:distributed_safe_at quorums ballot vote for ballot vote .
 
-definition amp_asig where
-  "amp_asig \<equiv>
-    \<lparr> inputs = { Propose c | c . True},
-      outputs = { Learn i v l | i v l . True},
-      internals = {Internal}\<rparr>"
-
-definition amp_start where
+definition start_s where
   -- {* The initial state *}
-  "amp_start \<equiv> {\<lparr>propCmd = {}, ballot = (\<lambda> a . 0), vote = (\<lambda> a i. Map.empty), 
-    suggestion = (\<lambda> i . Map.empty), onebs = \<lambda> a . Map.empty, learned = \<lambda> l . Map.empty,
-    leader = \<lambda> a . leading 0 = a\<rparr>}"
+  "start_s \<equiv> \<lparr>propCmd = {}, ballot = (\<lambda> a . 0), vote = (\<lambda> a i . Map.empty), 
+    suggestion = \<lambda> i . Map.empty, onebs = \<lambda> a . Map.empty,
+    inst_status = \<lambda> b . if b = 0 then Some Map.empty else None\<rparr>"
 
+definition start where "start \<equiv> {start_s}"
+  
 subsection {* The transitions *}
 
 definition propose where
   "propose c r r' \<equiv> (r' = r\<lparr>propCmd := (propCmd r) \<union> {c}\<rparr>)"
 
 definition join_ballot where
-  "join_ballot a b s s' \<equiv> 
-    let onebs' = \<lambda> i . distributed_safe_at.acc_max (\<lambda>a. vote s a i) a b
+  "join_ballot a b s s' \<equiv>
+    let onebs' = \<lambda> i . dsa.acc_max (flip (vote s) i) a b
     in
-      b > (ballot s a) 
+      b > (ballot s a)
       \<and> s' = s\<lparr>ballot := (ballot s)(a := b),
-        onebs := (onebs s)(a := (onebs s a)(b := Some onebs')),
-        leader := (amp_state.leader s)(a := False)\<rparr>"
+        onebs := (onebs s)(a := (onebs s a)(b \<mapsto> onebs'))\<rparr>"
+  
+definition join_started_ballot where "join_started_ballot a b s s' \<equiv>
+  inst_status s b \<noteq> None 
+  \<and> ballot s a < b
+  \<and> s' = s\<lparr>ballot := (ballot s)(a := b)\<rparr>"
+  
+definition max_vote where max_vote_def:
+  "max_vote s i b q \<equiv> max_by_key (\<Union> a \<in> q . the (onebs s a b) i) snd"
 
+definition sugg where sugg_def: "sugg s i b q \<equiv>
+  let m = max_vote s i b q in if m = {} then None else Some (the_elem (fst ` m))"
+  
+definition joined where "joined s q b \<equiv> \<forall> a \<in> q . onebs s a b \<noteq> None"
+  
 definition acquire_leadership where
-  "acquire_leadership a q s s' \<equiv> let b = ballot s a in 
-    leading b = a
+  -- {* Upon acquiring leadership, the leader makes suggestions in an
+  arbitrary set of instances which have a unique safe value. *}
+  "acquire_leadership a q s s' \<equiv> let b = ballot s a in
+    leader b = a
     \<and> q \<in> quorums
-    \<and> \<not> amp_state.leader s a 
-    \<and> (\<forall> a \<in> q . onebs s a b \<noteq> None)
-    \<and> s' = s\<lparr>leader := (amp_state.leader s)(a := True), 
-        suggestion := (\<lambda>i . (suggestion s i)(b :=
-          let m = distributed_safe_at.max_pair q (\<lambda> a . (the (onebs s a b)) i) in
-            map_option fst m))\<rparr>"
+    \<and> joined s q b
+    \<and> inst_status s b = None
+    \<and> inst_status s' = (inst_status s)(b := Some (\<lambda> i . sugg s i b q))
+    \<and> (\<forall> i . suggestion s' i = (suggestion s i)(b := sugg s i b q) 
+      \<or> suggestion s' i = (suggestion s i))
+    \<and> propCmd s' = propCmd s \<and> ballot s' = ballot s \<and> vote s' = vote s \<and> onebs s' = onebs s"
 
 definition suggest where "suggest a i b v s s' \<equiv>
           v \<in> propCmd s
         \<and> ballot s a = b
-        \<and> amp_state.leader s a
         \<and> suggestion s i b = None
-        \<and> s' = s\<lparr>suggestion := (suggestion s)(i := (suggestion s i)(b := Some v))\<rparr>"
+        \<and> (case inst_status s b of Some f \<Rightarrow> f i = None | _ \<Rightarrow> False)
+        \<and> s' = s\<lparr>suggestion := (suggestion s)(i := (suggestion s i)(b \<mapsto> v))\<rparr>"
 
 definition do_vote where
   "do_vote a i v s s' \<equiv> let b = ballot s a in
@@ -84,49 +79,48 @@ definition do_vote where
         \<and> suggestion s i b = Some v
         \<and> s' = s\<lparr>vote := (vote s)(a := (vote s a)(i := (vote s a i)(b := Some v)))\<rparr>"
 
-abbreviation chosen where
-  "chosen s i v \<equiv> ballot_array.chosen quorums (\<lambda>a. vote s a i) v"
+definition chosen where
+  "chosen s i v \<equiv> ballot_array.chosen quorums (flip (vote s) i) v"
 
 definition learn where
-  "learn l i v s s' \<equiv> chosen s i v \<and> 
-    s' = s\<lparr>learned := (learned s)(l := (learned s l)(i := Some v))\<rparr>"
+  "learn i v s s' \<equiv> chosen s i v \<and> s' = s"
+  
+definition re_join where 
+  "re_join a s s' \<equiv> True"
 
-definition catch_up where
-  "catch_up l1 l2 i v s s' \<equiv> learned s l2 i = Some v 
-    \<and> s' = s\<lparr>learned := (learned s)(l1 := (learned s l1)(i := Some v))\<rparr>"
-
-fun amp_trans_rel where
-  "amp_trans_rel r (Propose c) r' = propose c r r'"
-| "amp_trans_rel r Internal r' = (
+fun trans_rel where
+  "trans_rel r (Propose c) r' = propose c r r'"
+| "trans_rel r Internal r' = (
     (\<exists> a b . join_ballot a b r r')
     \<or> (\<exists> a i v . do_vote a i v r r')
     \<or> (\<exists> a i b v . suggest a i b v r r')
-    \<or> (\<exists> l1 l2 i v . catch_up l1 l2 i v r r')
-    \<or> (\<exists> a q . acquire_leadership a q r r'))"
-| "amp_trans_rel r (Learn i v l) r' = learn l i v r r'"
+    \<or> (\<exists> a q . acquire_leadership a q r r')
+    \<or> (\<exists> a b . join_started_ballot a b r r') )"
+| "trans_rel r (Learn i v) r' = learn i v r r'"
 
-lemma trans_cases[consumes 1]:
-  assumes "amp_trans_rel r a r'"
+lemma trans_cases:
+  assumes "trans_rel r a r'"
   obtains 
   (propose) c where "propose c r r'"
-| (learn) l i v where "learn l i v r r'"
+| (learn) i v where "learn i v r r'"
 | (join_ballot) a b where "join_ballot a b r r'"
 | (do_vote) a i v where "do_vote a i v r r'"
 | (suggest) a i b v where "suggest a i b v r r'"
-| (catch_up) l1 l2 i v where "catch_up l1 l2 i v r r'"
 | (acquire) a q where "acquire_leadership a q r r'"
-using assms by induct auto
+| (join_started) a b where "join_started_ballot a b r r'"
+  using assms apply induct apply simp
+  by (metis ampr1_ioa.trans_rel.simps(1) ampr1_ioa.trans_rel.simps(3) paxos_action.exhaust trans_rel.simps(2)) 
 
-definition amp_trans where
-  "amp_trans \<equiv> { (r,a,r') . amp_trans_rel r a r'}"
+definition trans where
+  "trans \<equiv> { (r,a,r') . trans_rel r a r'}"
 
 subsection {* The I/O-automaton *}
 
-definition amp_ioa where
-  "amp_ioa \<equiv> \<lparr>ioa.asig = amp_asig, start = amp_start, trans = amp_trans\<rparr>"
+definition ioa where
+  "ioa \<equiv> \<lparr>ioa.asig = paxos_asig, start = start, trans = trans\<rparr>"
 
-lemmas simps = amp_ioa_def amp_asig_def amp_start_def amp_trans_def propose_def join_ballot_def 
-  do_vote_def learn_def
+lemmas simps = ioa_def paxos_asig_def start_def trans_def propose_def join_ballot_def
+  do_vote_def learn_def suggest_def acquire_leadership_def
 
 end
 
