Isabelle2/AbstractMultiPaxosR1Correctness.thy
@@ -1,349 +1,318 @@
 section {* Proof of the agreement property of AbstractMultiPaxos. *}
 
 theory AbstractMultiPaxosR1Correctness
-imports AbstractMultiPaxosR1 "../../IO-Automata/IOA_Automation"
+imports AbstractMultiPaxosR1 IOA_Automation
   BallotArrayProperties
 begin
 
-locale amp_proof = IOA + quorums quorums + amp_ioa quorums for
+locale ampr1_proof = IOA + quorums quorums + ampr1_ioa quorums for
      quorums :: "'a set set" +
-  fixes the_ioa :: "(('v,'a,'l)amp_state, ('v,'a,'l)amp_action) ioa"
-  defines "the_ioa \<equiv> amp_ioa"
+  fixes the_ioa :: "(('v, 'a, 'l) ampr1_state, 'v paxos_action) ioa"
+  defines "the_ioa \<equiv> ioa"
 begin
+
+interpretation dsa_p:dsa_properties quorums ballot vote for ballot :: "'a \<Rightarrow> bal" 
+  and vote :: "'a \<Rightarrow> nat \<Rightarrow> 'v option"
+  by (unfold_locales)
 
 subsection {* Automation setup *}
 
-lemmas amp_ioa_defs =
-   is_trans_def actions_def amp_trans_def amp_start_def
-   externals_def amp_ioa_def amp_asig_def
-
-declare amp_ioa_defs[inv_proofs_defs]
-declare the_ioa_def[inv_proofs_defs]
+lemmas ioa_defs =
+   is_trans_def actions_def trans_def start_def start_s_def
+   externals_def ioa_def asig_def the_ioa_def
 
 declare propose_def[simp] join_ballot_def[simp] do_vote_def[simp] suggest_def[simp]
-  learn_def[simp] Let_def[simp] split_if[split] split_if_asm[split] catch_up_def[simp]
-  acquire_leadership_def[simp]
+  learn_def[simp] Let_def[simp] if_splits[split] acquire_leadership_def[simp]
+  join_started_ballot_def[simp]
+
+named_theorems inv_defs
 
 (*  Nitpick config:
 nitpick[no_assms, show_consts, verbose, card 'a = 3, card 'v = 2, card nat = 2, card "'v option" = 3, card "nat option" = 3,
-    card "('v \<times> nat) option" = 5, card "'v \<times> nat" = 4, card unit = 1, card "('v, 'a) amp_state" = 32]
+    card "('v \<times> nat) option" = 5, card "'v \<times> nat" = 4, card unit = 1, card "('v, 'a) ampr1_state" = 32]
 *)
+
 method rm_trans_rel_assm = 
-  (match premises in P[thin]:"amp_trans_rel ?x ?y ?z" \<Rightarrow> \<open>-\<close>)
-method unfold_to_trans_rel = 
-  (simp add:is_trans_def the_ioa_def amp_ioa_def amp_trans_def)
+  (match premises in P[thin]:"trans_rel ?x ?y ?z" \<Rightarrow> \<open>-\<close>)
 
-subsection {* Auxiliary invariants *}
+lemma is_trans_simp[simp]:
+  "s \<midarrow>a\<midarrow>the_ioa\<longrightarrow> t = trans_rel s a t"
+  by (simp add:is_trans_def the_ioa_def ioa_def trans_def)
+  
+method my_fail for msg::"char list" = (print_term msg; fail)
 
-definition inv6 where inv6_def[inv_proofs_defs]:
-  "inv6 s \<equiv> \<forall> a b i . leading b = a \<and> (ballot s a < b \<or> (ballot s a = b \<and> \<not> amp_state.leader s a))
+text {* If any of m1, m2, or m3 fail, then the whole method fails. *}
+method inv_cases methods m1 m2 m3 uses invs declares inv_defs =
+  (rule invariantI; (
+      ((match premises in "?s \<in> ioa.start ?ioa" \<Rightarrow> \<open>-\<close>); m1 )
+    | ((instantiate_invs_2 invs:invs | my_fail "''instantiation failed''");
+        (m2 | my_fail "''method 2 failed''"); simp only:is_trans_simp;
+          ((induct_tac rule:trans_cases | my_fail "''case analysis failed''"), simp?); rm_trans_rel_assm; m3)
+        ) )
+
+method force_inv uses invs declares inv_defs =
+  inv_cases \<open>(force simp add:inv_defs ioa_defs)?\<close> \<open>-\<close> \<open>(force simp add:inv_defs split:option.splits)?\<close>
+  invs:invs inv_defs:inv_defs
+
+method simp_inv uses invs declares inv_defs =
+  inv_cases \<open>simp add:inv_defs ioa_defs\<close> \<open>-\<close> \<open>(simp add:inv_defs split:option.splits; fail)?\<close>
+  invs:invs inv_defs:inv_defs
+
+subsection {* Invariants *}
+
+definition inv3 where inv3_def[inv_defs]:
+  -- {* acceptors only vote for the suggestion. *}
+  "inv3 s \<equiv> \<forall> i a b . let v = vote s a i b in v \<noteq> None \<longrightarrow> v = suggestion s i b"
+  
+context begin
+  -- {* Proof of @{term inv3} *}
+
+private definition inv1 where inv1_def[inv_defs]:
+  "inv1 s \<equiv> \<forall> b . inst_status s b \<noteq> None \<longrightarrow> ballot s (leader b) \<ge> b"
+  
+private lemma inv1: "invariant the_ioa inv1" by (force_inv)
+
+private definition inv2 where inv2_def[inv_defs]:
+  "inv2 s \<equiv> \<forall> a b i . leader b = a \<and> (ballot s a < b \<or> (ballot s a = b \<and> inst_status s b = None))
     \<longrightarrow> suggestion s i b = None"
 
-definition inv7 where inv7_def[inv_proofs_defs]:
-  "inv7 s \<equiv> \<forall> a . amp_state.leader s a \<longrightarrow> leading (ballot s a) = a"
+private lemma inv2: "invariant the_ioa inv2"
+  apply (simp_inv invs:inv1)
+   apply (simp add:ioa_defs inv_defs; case_tac s; case_tac t; force split:option.splits)
+  apply (simp add:ioa_defs inv_defs; case_tac s; case_tac t; simp) by (metis fun_upd_apply)
 
-lemma inv7: "invariant the_ioa inv7"
-apply (rule invariantI)
-apply (force simp add:inv_proofs_defs)
-apply (unfold_to_trans_rel)
-apply (rm_reachable)
-apply ((induct_tac rule:trans_cases, simp); rm_trans_rel_assm)
-apply (auto simp add:inv_proofs_defs)
-done
-declare inv7[invs]
+lemma inv3: "invariant the_ioa inv3" 
+  apply (simp_inv invs:inv2)
+   apply (simp add:ioa_defs inv_defs; case_tac s; case_tac t; force)
+  apply (simp add:ioa_defs inv_defs; case_tac s; case_tac t; auto split:option.splits)
+  by (metis fun_upd_apply option.distinct(1))
 
-lemma inv6: "invariant the_ioa inv6"
-apply (rule invariantI)
-apply (force simp add:inv_proofs_defs)
-apply instantiate_invs_2
-apply (unfold_to_trans_rel)
-apply ((induct_tac rule:trans_cases, simp); rm_trans_rel_assm)
-apply (auto simp add:inv_proofs_defs)
-done
-declare inv6[invs]
+end
 
-definition inv1 where inv1_def[inv_proofs_defs]:
-  -- {* acceptors only vote for the suggestion. *}
-  "inv1 s \<equiv> \<forall> a i b . let v = vote s a i b in v \<noteq> None \<longrightarrow> v = suggestion s i b"
+definition conservative where
+  "conservative s \<equiv>  \<forall> i . ballot_array.conservative_array (flip (vote s) i)"
 
-lemma inv1:
-  "invariant the_ioa inv1"
-apply (rule invariantI)
-apply (force simp add:inv_proofs_defs invs)
-apply instantiate_invs_2
-apply (unfold_to_trans_rel)
-apply ((induct_tac rule:trans_cases, simp); rm_trans_rel_assm)
-              apply (simp_all add:inv1_def)
-    apply (metis option.simps(3))
-  apply (simp add:inv7_def inv6_def)
-  apply force
-done
-declare inv1[invs]
-
-
-declare
-  ballot_array.conservative_array_def[inv_proofs_defs]
-  ballot_array.conservative_def[inv_proofs_defs]
-
-abbreviation conservative_array where
-  "conservative_array s \<equiv>  \<forall> i . ballot_array.conservative_array (\<lambda>a. vote s a i)"
-
-lemma conservative: "invariant the_ioa conservative_array"
+lemma conservative: "invariant the_ioa conservative"
 proof -
-  have "\<And> s . inv1 s \<Longrightarrow> conservative_array s"
-    by (auto simp add:inv_proofs_defs split add:option.splits) (metis option.sel)
-  with inv1 show ?thesis  using IOA.invariant_def by blast 
+  have "\<And> s . inv3 s \<Longrightarrow> conservative s"
+    apply (simp add:inv_defs ballot_array.conservative_def ballot_array.conservative_array_def
+       conservative_def split:option.splits) by (metis option.inject)
+  with inv3 show ?thesis  using IOA.invariant_def by blast
 qed
-declare conservative[invs]
 
-lemma trans_imp_prefix_order:
-  assumes "s \<midarrow>a\<midarrow>the_ioa\<longrightarrow> t"
-  shows "is_prefix (ballot s) (ballot t) (\<lambda>a. vote s a i) (\<lambda>a. vote t a i)" using assms
-  apply (simp add:inv_proofs_defs)
-  apply (induct rule:trans_cases)
-  apply (auto simp add:is_prefix_def inv_proofs_defs split add:option.split_asm)
-done
-
-abbreviation safe_at where "safe_at s i \<equiv> ballot_array.safe_at quorums (ballot s) (\<lambda>a. vote s a i)"
+definition safe_at where "safe_at s i \<equiv> dsa.safe_at (ballot s) (flip (vote s) i)"
 
 lemma safe_mono:
-  -- {* @{term safe_at} is monotonic. *}
+  -- {* @{term safe_at} is monotonic. A key lemma to simplify invariant proofs. *}
   assumes "s \<midarrow>a\<midarrow>the_ioa\<longrightarrow> t" and "safe_at s i v b"
-  shows "safe_at t i v b" using assms ballot_array_prefix.safe_at_mono
-by (metis ballot_array_prefix_axioms_def ballot_array_prefix_def quorums_axioms trans_imp_prefix_order) 
-
-definition inv3 where inv3_def[inv_proofs_defs]:
-  "inv3 s \<equiv> \<forall> a b . case onebs s a b of None \<Rightarrow> True
-    | Some maxs \<Rightarrow> 
-      (\<forall> i . maxs i = distributed_safe_at.acc_max (\<lambda>a. vote s a i) a b)
-      \<and> (ballot s a \<ge> b)"
-
-lemma inv3:
-  "invariant the_ioa inv3"
-apply (rule invariantI)
-apply (force simp add:inv_proofs_defs)
-apply instantiate_invs_2
-apply (unfold_to_trans_rel)
-apply ((induct_tac rule:trans_cases, simp); rm_trans_rel_assm)
-          apply (auto simp add:inv_proofs_defs split add:option.splits)[2]
-      defer defer apply (auto simp add:inv_proofs_defs split add:option.splits)[3]
-    defer
-    subgoal premises prems for s t act a i v
-    proof -
-      { fix a2 b maxs
-        assume a1:"onebs s a2 b = Some maxs"
-        from a1 prems(1) have 1:"\<And> j . maxs j = distributed_safe_at.acc_max (\<lambda>a. vote s a j) a2 b" 
-          by (simp add:inv3_def split add:option.splits split_if split_if_asm)
-        from a1 \<open>inv3 s\<close> \<open>do_vote a i v s t\<close> have 2:"ballot t a2 \<ge> b" by (simp add:inv3_def split add:option.splits)
-        { fix j assume "j \<noteq> i \<or> a \<noteq> a2"
-          hence "maxs j = distributed_safe_at.acc_max (\<lambda>a. vote t a j) a2 b" using 1 \<open>do_vote a i v s t\<close> by (auto simp add:distributed_safe_at.acc_max_def) }
-        note 3 = this
-        { fix j assume "j = i \<and> a = a2"
-          hence "maxs j = distributed_safe_at.acc_max (\<lambda>a. vote t a j) a2 b" using 1 \<open>do_vote a i v s t\<close> a1 2 apply (simp add:distributed_safe_at.acc_max_def)
-            by (smt Collect_cong amp_state.select_convs(2) amp_state.surjective amp_state.update_convs(3) dual_order.strict_trans1 neq_iff split_cong) }
-        note this 2 3 }
-      thus ?thesis apply (simp add:inv3_def split add:option.splits)
-        by (metis (no_types, lifting) amp_ioa.do_vote_def amp_state.select_convs(5) amp_state.surjective amp_state.update_convs(3) \<open>do_vote a i v s t\<close>)
-    qed
-  apply (auto simp add:inv_proofs_defs split add:option.splits)
-  apply (meson dual_order.trans less_imp_le_nat)
-done
-declare inv3[invs]
-      
-(* nitpick[no_assms, show_consts, verbose, card 'a = 3, card 'v = 2, card nat = 2, card "'v option" = 3, card "nat option" = 3,
-    card "('v \<times> nat) option" = 5, card "'v \<times> nat" = 4, card unit = 1, card "('v, 'a) amp_state" = 32, card 'l = 1, expect=none]  *)
-
-abbreviation safe where "safe s \<equiv> \<forall> i . ballot_array.safe quorums (ballot s) (\<lambda>a. vote s a i)"
-declare ballot_array.safe_def[inv_proofs_defs]
-
-lemma aqcuire_leadership_ok:
-  assumes "acquire_leadership a q s t" and "inv3 s" and "safe s" and "conservative_array t"
-  shows "let safe_at = \<lambda> v . ballot_array.safe_at quorums (ballot t) (\<lambda>a. vote t a i) v (ballot t a) in
-    case suggestion t i (ballot t a) of Some v \<Rightarrow> safe_at v | None \<Rightarrow> safe_at v"
+  shows "safe_at t i v b"
 proof -
-  let ?b = "ballot s a"
-  have 2:"?b = ballot t a" using assms(1) by (auto simp add:inv_proofs_defs)
-  let ?proved_safe_at = "distributed_safe_at.proved_safe_at quorums (ballot t) (\<lambda>a. vote t a i) q ?b"
-  have 5:"case suggestion t i (ballot t a) of Some v \<Rightarrow>  ?proved_safe_at v | None \<Rightarrow> ?proved_safe_at v"
-  proof -  
-    have "q \<in> quorums" by (metis acquire_leadership_def assms(1)) 
-    moreover
-    have "\<And> a2 . a2 \<in> q \<Longrightarrow> ?b \<le> ballot t a2" using assms(1,2) apply (auto simp add:inv_proofs_defs) by (metis (no_types, lifting) option.simps(5))
-    moreover
-    have "distributed_safe_at.max_pair q (\<lambda> a2 . the (onebs t a2 ?b) i) = 
-      distributed_safe_at.max_pair q (\<lambda> a2 . distributed_safe_at.acc_max (\<lambda>a. vote t a i) a2 ?b)"
-    proof -
-      have "distributed_safe_at.max_pair q (\<lambda> a2 . the (onebs s a2 ?b) i) = 
-        distributed_safe_at.max_pair q (\<lambda> a2 . distributed_safe_at.acc_max (\<lambda>a. vote s a i) a2 ?b)"
-      proof -
-        have "\<And> a2 . a2 \<in> q \<Longrightarrow> case onebs s a2 ?b of 
-                  Some f \<Rightarrow> f i = distributed_safe_at.acc_max (\<lambda>a. vote s a i) a2 ?b 
-                | None \<Rightarrow> False" using assms by (auto simp add:inv_proofs_defs split add:option.splits)
-        thus ?thesis apply (simp add:distributed_safe_at.max_pair_def split add:option.splits) by (smt SUP_cong option.case_eq_if)
-      qed
-      thus ?thesis using assms(1) by (auto simp add:inv_proofs_defs)
-    qed
-    ultimately show ?thesis using assms(1) by (auto simp add:distributed_safe_at.proved_safe_at_def split add:option.splits)
-  qed
-  have 6:"safe t" using assms(1) assms(3) by (auto simp add:inv_proofs_defs)
-  interpret p:dsa_properties "ballot t" "\<lambda>a. vote t a i" quorums by unfold_locales
-  show ?thesis using 2 5 6 p.proved_safe_at_imp_safe_at assms(4) by (metis option.case_eq_if option.distinct(1) option.sel p.safe_def)
+  have "is_prefix (ballot s) (ballot t) (flip (vote s) i) (flip (vote t) i)" using \<open>s \<midarrow>a\<midarrow>the_ioa\<longrightarrow> t\<close>
+    by (simp add:inv_defs ioa_defs; induct_tac rule:trans_cases, auto simp add:is_prefix_def inv_defs split:option.split_asm)
+  thus ?thesis
+  using assms ballot_array_prefix.safe_at_mono unfolding safe_at_def
+  by (metis ballot_array_prefix_axioms_def ballot_array_prefix_def quorums_axioms) 
 qed
 
-definition inv8 where inv8_def[inv_proofs_defs]:
-  "inv8 s \<equiv> \<forall> a i v . let b = ballot s a in
-    amp_state.leader s a \<and> suggestion s i b = None \<longrightarrow> safe_at s i v b"
+method insert_safe_mono =
+  match premises in P:"?s \<midarrow>?a\<midarrow>the_ioa\<longrightarrow> ?t" \<Rightarrow> \<open>insert safe_mono[OF P]\<close>
+method inv_cases_3 uses invs declares inv_defs =
+  inv_cases \<open>-\<close> \<open>insert_safe_mono\<close> \<open>-\<close> invs:invs inv_defs:inv_defs
 
-definition inv2 where
-  -- {* a suggestion is safe. *}
-  inv2_def[inv_proofs_defs]:"inv2 s \<equiv> \<forall> i b . case suggestion s i b of Some v \<Rightarrow> safe_at s i v b | None \<Rightarrow> True"
+definition safe where "safe s \<equiv> \<forall> a i b . case vote s a i b of Some v \<Rightarrow> safe_at s i v b | _ \<Rightarrow> True"
 
-lemma inv8_inv2_safe:"invariant the_ioa (\<lambda> s . inv8 s \<and> inv2 s \<and> safe s)"
-apply (rule invariantI)
-    apply (force simp add:inv_proofs_defs ballot_array.safe_at_def)
-  apply instantiate_invs_2
-  subgoal premises prems for s t act
-  proof -
-    note safe_mono[OF prems(2)]
-    thus ?thesis using prems 
-    apply (unfold_to_trans_rel)
-    apply ((induct_tac rule:trans_cases, simp); rm_trans_rel_assm)
-                  apply (auto simp add:inv_proofs_defs split add:option.splits)[3]
-            defer
-            apply (auto simp add:inv_proofs_defs split add:option.splits)[2]
-            apply (elim conjE)
-        subgoal premises prems for a q
-        proof (rule conjI; (rule conjI)?) thm prems
-          show "safe t" using \<open>safe s\<close> \<open>acquire_leadership a q s t\<close> by (auto simp add:inv_proofs_defs)
-        next
-          show "inv8 t"  proof (auto simp add:inv8_def)
-            fix a2 i v
-            assume a1:"amp_state.leader t a2" and a2:"suggestion t i (ballot t a2) = None"
-            show "safe_at t i v (ballot t a2)"
-            proof (cases "a2 = a")
-              case False thus ?thesis using \<open>acquire_leadership a q s t\<close> \<open>inv8 s\<close> \<open>inv7 s\<close> prems(1) a1 a2
-                by (fastforce simp add:inv_proofs_defs)
-            next
-              case True thus ?thesis using aqcuire_leadership_ok \<open>inv3 s\<close> \<open>safe s\<close> \<open>\<forall>i. ballot_array.conservative_array (\<lambda>a. vote t a i)\<close> 
-                \<open>acquire_leadership a q s t\<close> a2 by (metis case_optionE option.simps(3))
-            qed
-          qed
-        next
-          show "inv2 t" proof (auto simp add:inv2_def split add:option.splits)
-            fix i b v
-            assume a1:"suggestion t i b = Some v"
-            show "safe_at t i v b"
-            proof (cases "b = ballot s a")
-              case False thus ?thesis using \<open>acquire_leadership a q s t\<close> \<open>inv2 s\<close> prems(1) a1 \<open>inv7 s\<close> 
-                by (auto simp add:inv_proofs_defs split add:option.splits)
-            next
-              case True 
-              have 1:"ballot t = ballot s" using \<open>acquire_leadership a q s t\<close> by simp
-              show ?thesis using 1 True aqcuire_leadership_ok[OF \<open>acquire_leadership a q s t\<close> \<open>inv3 s\<close> \<open>safe s\<close> \<open>\<forall>i. ballot_array.conservative_array (\<lambda>a. vote t a i)\<close>, of i]  
-                a1 \<open>inv7 s\<close> by (fastforce simp only:inv7_def Let_def split add:option.splits)
-            qed
-          qed
-        qed
-        
-      apply (elim conjE)
-      subgoal premises prems for a i v
-      proof (rule conjI; (rule conjI)?) thm prems(12,14,9)
-        show "inv8 t" using \<open>inv8 s\<close> \<open>do_vote a i v s t\<close> unfolding amp_ioa.do_vote_def inv8_def
-          by (smt amp_state.ext_inject amp_state.surjective amp_state.update_convs(3) prems(1))
-      next
-        show "inv2 t" using prems(1) \<open>inv2 s\<close> \<open>do_vote a i v s t\<close> unfolding amp_ioa.do_vote_def inv2_def 
-          by (smt amp_state.ext_inject amp_state.surjective amp_state.update_convs(3) option.case_eq_if) 
-      next
-        show "safe t" using prems(1) \<open>do_vote a i v s t\<close> \<open>inv2 s\<close> \<open>inv1 t\<close> unfolding amp_ioa.do_vote_def ballot_array.safe_def inv1_def inv2_def 
-          by (smt amp_state.ext_inject amp_state.surjective amp_state.update_convs(3) option.case_eq_if ) 
-      qed
+definition inv4 where inv4_def[inv_defs]:"inv4 s \<equiv> \<forall> i b . 
+  case suggestion s i b of Some v \<Rightarrow> 
+    (case inst_status s b of Some f \<Rightarrow>
+      (case f i of None \<Rightarrow> True | Some w \<Rightarrow> v = w)
+    | None \<Rightarrow> False)
+  | None \<Rightarrow> True"
+  
+lemma inv4:"invariant the_ioa inv4"
+  apply (simp_inv; (simp add:ioa_defs inv_defs; case_tac s; case_tac t; clarify; simp split:option.splits))
+      apply (metis option.collapse option.distinct(1))
+     apply (metis option.collapse option.distinct(1)) 
+    apply (metis option.collapse option.distinct(1)) 
+   apply auto
+      apply fastforce
+     apply (metis option.collapse option.distinct(1))
+    apply (metis fun_upd_apply option.distinct(1) option.inject)
+    apply (metis fun_upd_apply option.distinct(1))
+   apply (metis fun_upd_apply)
+  by (metis option.collapse option.distinct(1))
+
+definition inst_status_inv where inst_status_inv_def[inv_defs]:
+  "inst_status_inv s \<equiv> (\<forall> b . case inst_status s b of Some f \<Rightarrow> 
+    (\<forall> i . case f i of Some v \<Rightarrow> safe_at s i v b | None \<Rightarrow> (\<forall> v . safe_at s i v b))
+    | None \<Rightarrow> True)"
+
+definition the_inv where the_inv_def[inv_defs]: "the_inv s \<equiv> 
+  safe s  \<and> inst_status_inv s"
+  
+context begin
+  --{* Proof of @{term the_inv} *}
+
+private
+definition inv5 where inv5_def[inv_defs]:"inv5 s \<equiv> \<forall> a b f i . onebs s a b = Some f 
+      \<longrightarrow> f i = dsa.acc_max (flip (vote s) i) a b \<and> ballot s a \<ge> b"
+
+private
+lemma inv5:"invariant the_ioa inv5"
+  -- {* The @{term do_vote} case necessitates to show that the value of @{term dsa.acc_max} dose not change as a result of the vote.  *}
+  apply (force_inv inv_defs:inv5_def)
+  subgoal premises prems for s t _ a2 i2 v unfolding inv5_def
+      -- {* the @{term do_vote} case *}
+  proof (clarify, rule conjI)
+    fix a b f i
+    assume "onebs t a b = Some f"
+    hence "onebs s a b = Some f" using \<open>do_vote a2 i2 v s t\<close> unfolding do_vote_def by auto
+    hence "f i = dsa.acc_max (flip (vote s) i) a b" and "b \<le> ballot s a" using \<open>inv5 s\<close> unfolding inv5_def by auto
+    have "dsa.acc_max (flip (vote t) i) a b = dsa.acc_max (flip (vote s) i) a b"
+    proof -
+      from \<open>b \<le> ballot s a\<close> have "\<And> b' . b' < b \<Longrightarrow> flip (vote s) i a b' = flip (vote t) i a b'" using  \<open>do_vote a2 i2 v s t\<close>
+        unfolding do_vote_def by auto
+      hence "{(v, ba). ba < b \<and> flip (vote s) i a ba = Some v} = {(v, ba). ba < b \<and> flip (vote t) i a ba = Some v}" by metis
+      thus ?thesis unfolding dsa.acc_max_def dsa.a_votes_def by auto
+    qed
+    with \<open>f i = dsa.acc_max (flip (vote s) i) a b\<close> show "f i = dsa.acc_max (flip (vote t) i) a b" by auto
+    from \<open>b \<le> ballot s a\<close> and \<open>do_vote a2 i2 v s t\<close> show "b \<le> ballot t a" unfolding do_vote_def by auto
+  qed
+  done
+
+  
+lemma the_inv:"invariant the_ioa the_inv"
+  apply (inv_cases_3 invs:inv4 conservative inv5)
+        apply (simp add:ioa_defs inv_defs safe_def ballot_array.safe_def safe_at_def dsa_p.safe_at_0)
+       apply (simp add:ioa_defs inv_defs safe_def split:option.splits)
+       apply (metis option.distinct(1))
+      apply (simp add:inv_defs split:option.splits)
+  subgoal premises prems for s t _ a b (* join_ballot *)
+  proof (auto simp add:the_inv_def)
+    from \<open>join_ballot a b s t\<close> have 1:"inst_status t = inst_status s" and 2:"vote t = vote s" by auto
+    note mono = \<open>(\<And>i v b. safe_at s i v b \<Longrightarrow> safe_at t i v b)\<close>
+    show "safe t" using \<open>the_inv s\<close>  2 mono
+      by (auto simp add:safe_def ballot_array.safe_def safe_at_def inv_defs split:option.splits)
+    show "inst_status_inv t" using 1 2 mono \<open>the_inv s\<close>
+      by (force simp add:inv_defs split:option.splits)
+  qed
+  subgoal premises prems for s t _ a i v (* do_vote *)
+  proof (auto simp add:the_inv_def)
+    note mono = \<open>(\<And>i v b. safe_at s i v b \<Longrightarrow> safe_at t i v b)\<close>
+    have 1:"\<And> i b v . suggestion s i b = Some v \<Longrightarrow> safe_at s i v b" using \<open>the_inv s\<close> \<open>inv4 s\<close>
+      by (fastforce simp add:safe_def inv_defs split:option.splits)
+    show "safe t" using \<open>the_inv s\<close> mono \<open>do_vote a i v s t \<close> 1
+      by (auto simp add:safe_def inv_defs split:option.splits)
+    show "inst_status_inv t" using \<open>the_inv s\<close> mono \<open>do_vote a i v s t \<close>
+      apply (cases s, cases t, auto simp add: inv_defs safe_def split!:option.splits)
+      by (metis option.distinct(1))
+  qed
+  subgoal for s t _ _ _ _ _ (* suggest *)
+    apply (cases s, cases t, auto simp add: inv_defs safe_def split:option.splits)[1]
+    apply (metis option.distinct(1))
     done
+  subgoal premises prems for s t _ a q (* acquire_leadership *)
+  proof (auto simp add:the_inv_def)
+    note mono = \<open>(\<And>i v b. safe_at s i v b \<Longrightarrow> safe_at t i v b)\<close>
+    show "safe t" using \<open>acquire_leadership a q s t\<close> \<open>the_inv s\<close> mono
+      by (auto simp add:safe_def inv_defs split:option.splits)
+    show "inst_status_inv t"
+    proof -
+      let ?b = "ballot s a"
+      from \<open>acquire_leadership a q s t\<close> have "joined s q ?b" and \<open>q\<in> quorums\<close> by (auto simp add:safe_def inv_defs split:option.splits)
+      from \<open>the_inv s\<close> have "safe s" by (simp add: the_inv_def) 
+      
+      text {* First we show that @{term max_vote} is the max over @{term dsa.acc_max} 
+        (i.e. @{term dsa.max_quorum_votes} *}
+      have 1:"max_vote s i ?b q = dsa.max_quorum_votes (flip (vote s) i) q ?b" for i 
+      proof -
+        have "(the (onebs s a ?b)) i = dsa.acc_max (flip (vote s) i) a ?b" if "a \<in> q" for a i
+          using \<open>inv5 s\<close> \<open>joined s q ?b\<close> that by (simp add: ampr1_ioa.joined_def inv5_def)
+        thus ?thesis by (auto simp add:max_vote_def dsa.max_quorum_votes_def)
+      qed
+      have 2:"ballot s a \<ge> ?b" if "a \<in> q" for a using \<open>joined s q ?b\<close> \<open>inv5 s\<close> that by (auto simp add:inv5_def joined_def)
+      
+      text {* Then we show that a suggestion is @{term dsa.proved_safe_at}, and that everything is 
+        safe if there is no suggestion *}
+      let ?proved="\<lambda> i . dsa.proved_safe_at (ballot s) (flip (vote s) i) q ?b"
+      have 3:"case sugg s i ?b q of Some v \<Rightarrow> ?proved i v | None \<Rightarrow> (\<forall> v . ?proved i v)" for i
+      proof (cases "sugg s i ?b q")
+        case None
+        hence "dsa.max_quorum_votes (flip (vote s) i) q ?b = {}" unfolding sugg_def
+            \<open>max_vote s i ?b q = dsa.max_quorum_votes (flip (vote s) i) q ?b\<close> by auto
+        thus ?thesis using 2 \<open>q \<in> quorums\<close> None unfolding dsa.proved_safe_at_def joined_def by auto 
+      next
+        case (Some v)
+          -- {* Here the difficulty lies in the use of @{term the_elem} in @{thm sugg_def} *}
+        obtain x where "dsa.max_quorum_votes (flip (vote s) i) q ?b = {x}"
+        proof -
+          from Some have "max_vote s i ?b q \<noteq> {}" unfolding sugg_def by auto
+          moreover
+          note \<open>max_vote s i ?b q = dsa.max_quorum_votes (flip (vote s) i) q ?b\<close>  and \<open>conservative s\<close> 
+          moreover note dsa_p.max_vote_e_or_singleton
+          ultimately show ?thesis using that unfolding conservative_def by (metis \<open>q \<in> quorums\<close>) 
+        qed
+        moreover 
+        have "v = (the_elem (fst ` (dsa.max_quorum_votes (flip (vote s) i) q ?b)))" using Some \<open>joined s q ?b\<close> 1
+          by (auto simp add: sugg_def)
+        ultimately show ?thesis using \<open>q\<in>quorums\<close> \<open>joined s q ?b\<close> 1 2 Some
+          unfolding dsa.proved_safe_at_def by auto
+      qed
+      
+      text {* Finally we conclude using lemma @{thm dsa_p.proved_safe_at_imp_safe_at} *}
+      
+      obtain f where 6:"f = (\<lambda> i . sugg s i ?b q)" and 7:"inst_status t (ballot s a) = Some f" using \<open>acquire_leadership a q s t\<close> 
+        using \<open>acquire_leadership a q s t\<close> by simp
+      have 8:"case f i of Some v \<Rightarrow> safe_at s i v ?b | None \<Rightarrow> safe_at s i v ?b" for i v
+      proof (cases "f i")
+        case None
+        with \<open>acquire_leadership a q s t\<close> 6 have "sugg s i ?b q = None" by auto
+        with 3 have "dsa.proved_safe_at (ballot s) (flip (vote s) i) q ?b v" by (metis (mono_tags) option.simps(4)) 
+        thus ?thesis using \<open>conservative s\<close> \<open>q\<in>quorums\<close> dsa_p.proved_safe_at_imp_safe_at None
+          apply (auto simp add:safe_def safe_at_def conservative_def split:option.splits)
+          apply (metis (full_types) ampr1_proof.safe_at_def ampr1_proof.safe_def ampr1_proof_axioms dsa.safe_def \<open>safe s\<close>)
+          done
+      next
+        case (Some w)
+        from Some 6 have 7:"sugg s i ?b q = Some w" by auto
+        hence "dsa.proved_safe_at (ballot s) (flip (vote s) i) q ?b w" using "3" by (metis option.simps(5)) 
+        with \<open>safe s\<close> and \<open>conservative s\<close> show ?thesis using Some \<open>q\<in>quorums\<close> dsa_p.proved_safe_at_imp_safe_at
+          by (auto simp add:safe_def safe_at_def conservative_def ballot_array.safe_def inv_defs split!:option.splits)
+      qed
+      from 7 8 show ?thesis using \<open>the_inv s\<close> \<open>acquire_leadership a q s t\<close> mono
+        apply (simp add: inv_defs split:option.splits)
+        by (smt option.case_eq_if option.distinct(1) option.sel)
+    qed
   qed
-done
-declare inv8_inv2_safe[invs]
+  apply (simp add:ioa_defs inv_defs safe_def split:option.splits; metis option.distinct(1))
+  done
+  
+end
 
-definition inv5 where
-  inv5_def[inv_proofs_defs]:"inv5 s \<equiv> \<forall> a i b . ballot s a < b \<longrightarrow> vote s a i b = None"
-
-lemma  inv5:"invariant the_ioa inv5"
-apply (rule invariantI)
-apply (force simp add:inv_proofs_defs)
-apply instantiate_invs_2
-apply (unfold_to_trans_rel)
-apply (induct_tac rule:trans_cases, simp)
-apply (auto simp add:inv_proofs_defs split add:option.splits)
-done
-declare inv5[invs]
-
-lemma chosen_mono: assumes "chosen s i v" and "s \<midarrow>a\<midarrow>the_ioa\<longrightarrow> t" and "inv5 s"
-  shows "chosen t i v" using assms
-apply (unfold_to_trans_rel)
-apply ((induct_tac rule:trans_cases, simp); rm_trans_rel_assm)
-apply (auto simp add:inv_proofs_defs split add:option.splits)[3] defer
-apply (auto simp add:inv_proofs_defs split add:option.splits)[1]
-apply (cases s, cases t, auto simp add:inv_proofs_defs ballot_array.chosen_def ballot_array.chosen_at_def split add:option.splits)
-apply (metis option.distinct(1)) by blast
-(* nitpick[no_assms, show_consts, verbose,expect=none unknown, card 'a = 3, card 'v = 2, card 'l = 1, card 'v option = 3, card nat = 2, card nat option = 3,
-  card "(nat \<Rightarrow> ('v \<times> nat) option) option" = 10, card "('v \<times> nat) option" = 5] *)
-
-definition inv4 where inv4_def[inv_proofs_defs]:
-  "inv4 s \<equiv> \<forall> i l . case learned s l i of Some v \<Rightarrow> chosen s i v | None \<Rightarrow> True"
-
-lemma  inv4:"invariant the_ioa inv4"
-apply (rule invariantI)
-apply (force simp add:inv_proofs_defs)
-apply instantiate_invs_2
-apply (unfold_to_trans_rel)
-apply (induct_tac rule:trans_cases, simp)
-apply (auto simp add:inv_proofs_defs split add:option.splits)[3] defer
-apply (auto simp add:inv_proofs_defs split add:option.splits)[1]
-apply (insert chosen_mono[simplified inv_proofs_defs])
-apply (auto simp add:inv4_def inv5_def split add:option.splits) 
-unfolding  ballot_array.chosen_def ballot_array.chosen_at_def
-proof -
-  fix s :: "('v, 'a, 'l) amp_state" and a :: "('v, 'a, 'l) amp_action" and aa :: 'a and i :: nat and v :: 'v and ia :: nat and l :: 'l and x2 :: 'v
-  assume a1: "\<forall>i l x2. learned s l i = Some x2 \<longrightarrow> (\<exists>b q. q \<in> quorums \<and> (\<forall>a\<in>q. vote s a i b = Some x2))"
-  assume a2: "vote s aa i (ballot s aa) = None"
-  assume a3: "learned s l ia = Some x2"
-  { fix aaa :: "nat \<Rightarrow> 'a set \<Rightarrow> 'a"
-    obtain AA :: "nat \<Rightarrow> 'l \<Rightarrow> 'v \<Rightarrow> 'a set" and nn :: "nat \<Rightarrow> 'l \<Rightarrow> 'v \<Rightarrow> nat" where
-      ff1: "\<forall>n l v. learned s l n \<noteq> Some v \<or> AA n l v \<in> quorums \<and> (\<forall>a. a \<notin> AA n l v \<or> vote s a n (nn n l v) = Some v)"
-      using a1 by (metis (no_types))
-    have "aaa (nn ia l x2) (AA ia l x2) = aa \<longrightarrow> (\<exists>n. (if aaa n (AA ia l x2) = aa then (vote s aa)(i := vote s aa i(ballot s aa \<mapsto> v)) else vote s (aaa n (AA ia l x2))) ia n = Some x2) \<or> (\<exists>n. vote s (aaa n (AA ia l x2)) ia (nn ia l x2) \<noteq> Some x2)"
-      using a2 by force
-    moreover
-    { assume "aaa (nn ia l x2) (AA ia l x2) \<noteq> aa"
-      then have "(\<exists>n. vote s (aaa n (AA ia l x2)) ia (nn ia l x2) \<noteq> Some x2) \<or> (\<exists>n. (if aaa n (AA ia l x2) = aa then (vote s aa)(i := vote s aa i(ballot s aa \<mapsto> v)) else vote s (aaa n (AA ia l x2))) ia n = Some x2)"
-        by force }
-    ultimately have "\<exists>n A. A \<in> quorums \<and> (aaa n A \<notin> A \<or> (if aaa n A = aa then (vote s aa)(i := vote s aa i(ballot s aa \<mapsto> v)) else vote s (aaa n A)) ia n = Some x2)"
-      using ff1 a3 by blast }
-  then show "\<exists>n A. A \<in> quorums \<and> (\<forall>a\<in>A. (if a = aa then (vote s aa)(i := vote s aa i(ballot s aa \<mapsto> v)) else vote s a) ia n = Some x2)"
-    by (metis (no_types))
-qed
-(*apply (metis (mono_tags) amp_state.select_convs(3) amp_state.surjective amp_state.update_convs(3) fun_upd_same)
-by (metis (mono_tags) amp_state.select_convs(3) amp_state.surjective amp_state.update_convs(3) fun_upd_same)*)
-declare inv4[invs]
-
-subsection {* Finally, the proof of agreement. *}
-
-definition agreement where agreement_def[inv_proofs_defs]:
-  "agreement s \<equiv> \<forall> i l1 l2 . let v = learned s l1 i; w = learned s l2 i 
-    in v \<noteq> None \<and> w \<noteq> None \<longrightarrow> v = w"
-
-lemma agreement:"invariant the_ioa agreement"
+definition inv7 where inv7_def[inv_defs]:
+  "inv7 s \<equiv> \<forall> i . ballot_array.safe quorums (ballot s) (flip (vote s) i)"
+  
+lemma inv7:"invariant the_ioa inv7"
 proof -
   { fix s
-    assume "inv4 s" and "safe s"
-    have "agreement s"
-    proof (auto simp add:inv_proofs_defs)
-      fix i l1 l2 v w
-      assume a1:"learned s l1 i = Some v" and a2:"learned s l2 i = Some w"
-      with \<open>inv4 s\<close> have "chosen s i v" and "chosen s i w" by (auto simp add:inv_proofs_defs split add:option.splits)
-      with \<open>safe s\<close> show "v = w" by (metis ballot_array_props.intro ballot_array_props.safe_imp_agreement quorums_axioms)
-    qed }
-  thus ?thesis using inv4 inv8_inv2_safe unfolding IOA.invariant_def by blast
+    assume "the_inv s" and "inv3 s" and "inv4 s"
+    hence "flip (vote s) i a b = Some v \<longrightarrow> safe_at s i v b" for a i b v  apply (simp add:inv_defs) by (metis (no_types) option.simps(5) safe_def)
+    hence "inv7 s"   by (simp add:ballot_array.safe_def safe_at_def inv7_def split:option.splits) }
+  thus ?thesis by (smt IOA.invariant_def inv4 inv3 the_inv) 
 qed
-    
+
+context begin
+-- {* Is this stuff needed? *}
+
+private
+definition inv6 where
+  inv6_def[inv_defs]:"inv6 s \<equiv> \<forall> i a b . ballot s a < b \<longrightarrow> flip (vote s) i a b = None"
+  
+private
+lemma  inv6:"invariant the_ioa inv6"
+by (force_inv)
+
+end
+
 end
 
 end
