Isabelle2/AbstractMultiPaxosR2.thy
@@ -1,99 +1,223 @@
 theory AbstractMultiPaxosR2
-imports  AbstractMultiPaxosR1Correctness "~~/src/HOL/Library/FinFun"
+imports  AbstractMultiPaxosR1 "~~/src/HOL/Library/FinFun"
 begin
 
-text {*
-1) Acceptors vote for a suggestion, and leaders use the distributed implementation of the safe-at computation.
-2) Explicit 1b messages.
-3) Explicit learning.
-4) Catch-up.
-5) Localizing suggestions (the leader function).
-6) Explicit leadership acquisition.
-7) Per-acceptor state.
-8) finfuns.
-*}
+text {* An executable version of R1 using finfun. *}
+
+unbundle finfun_syntax
+
+section {* A finfun-friendly definition of @{term acc_max} *}
+
+definition acc_max_2 where
+  "acc_max_2 (bound::nat) votes \<equiv> 
+    if (\<exists> b < bound . votes b \<noteq> None)
+    then Some (the_elem (max_by_key {(v,b) . b < bound \<and> votes b = Some v} snd))
+    else None"
+
+lemma acc_max_2_code[code]:
+  "acc_max_2 bound votes = (
+    if (\<exists> b < bound . votes b \<noteq> None)
+    then let votes = ((\<lambda> b . votes b \<bind> (\<lambda> v . Some (v,b))) ` {0..<bound}) \<bind> option_as_set in
+      Some (the_elem (max_by_key votes snd))
+    else None)" sorry
+
+lemma "acc_max_2 b (vote s i a) = acc_max (vote s i) a b"
+  by (auto simp add:acc_max_2_def acc_max_def distributed_safe_at.acc_max_def)
+
+lift_definition finfun_acc_max_2 :: "nat \<Rightarrow> (nat \<Rightarrow>f 'c option) \<Rightarrow> ('c \<times> nat) option"
+  is acc_max_2 .
+  -- {* Takes the ballot bound, and the votes per ballot. *}
+
+experiment
+begin
+
+text {* The restriction operator is not executable, so does not work. 
+TODO: could have used filter. *}
+
+lemma acc_max_2_code_2: 
+  "acc_max_2 bound votes = (
+    if (\<exists> b \<in> {0..<bound} . votes b \<noteq> None)
+    then let votes = ran ((\<lambda> b . votes b \<bind> (\<lambda> v . Some (v,b))) |` {0..<bound}) in
+      Some (the_elem (max_by_key votes snd))
+    else None)" oops
+  
+end
+
+section {* The IOA *}
 
 record ('v,'a,'l) ampr2_state =
   propCmd :: "'v set"
   ballot :: "'a \<Rightarrow>f bal"
-  vote :: "'a \<Rightarrow>f inst \<Rightarrow>f bal \<Rightarrow>f 'v option"
-  suggestion :: "inst \<Rightarrow> bal \<Rightarrow>f 'v option"
-  onebs :: "'a \<Rightarrow>f bal \<Rightarrow>f (inst \<Rightarrow> ('v\<times>bal) option) option"
+  vote :: "inst \<Rightarrow>f bal \<Rightarrow>f 'a \<Rightarrow>f 'v option"
+  suggestion :: "inst \<Rightarrow>f bal \<Rightarrow>f 'v option"
+  onebs :: "'a \<Rightarrow>f bal \<Rightarrow>f (inst \<Rightarrow>f ('v\<times>bal) option) option"
   learned :: "'l \<Rightarrow>f inst \<Rightarrow>f 'v option"
   leader :: "'a \<Rightarrow>f bool"
 
-locale ampr2_ioa = IOA + ampr1:amp_ioa quorums leading for quorums :: "'a set set" and leading
+locale ampr2_ioa = 
+  fixes quorums :: "'a set set" and leader :: "bal \<Rightarrow> 'a"
 begin
-
-definition asig where
-  "asig \<equiv>
-    \<lparr> inputs = { ampr1.Propose c | c . True},
-      outputs = { ampr1.Learn i v l | i v l . True},
-      internals = {ampr1.Internal}\<rparr>"
 
 definition start where
   -- {* The initial state *}
   "start \<equiv> {\<lparr>propCmd = {}, ballot = K$ 0, vote = K$ K$ K$ None, 
-    suggestion = \<lambda>i. (K$ None), onebs = K$ K$ None, learned = K$ K$ None,
-    leader = (K$ False)(leading 0 $:= True)\<rparr>}"
+    suggestion = K$ K$ None, onebs = K$ K$ None, learned = K$ K$ None,
+    leader = (K$ False)(leader 0 $:= True)\<rparr>}"
 
-subsection {* The transitions *}
+subsection {* propose and @{text join_ballot} *}
 
 definition propose where
   "propose c r r' \<equiv> (r' = r\<lparr>propCmd := (propCmd r) \<union> {c}\<rparr>)"
 
+notepad begin
+  fix vote::"inst \<Rightarrow>f bal \<Rightarrow>f 'a \<Rightarrow>f 'v option"
+  fix b :: bal
+  fix a :: 'a
+  define x1 where "x1 \<equiv> (op o$ (flip op$ a)) o$ vote"
+end
+  
 definition join_ballot where
-  "join_ballot a b s s' \<equiv> 
-    let onebs' = \<lambda>i. (distributed_safe_at.acc_max (\<lambda> a b. vote s $ a $ i $ b) a b)
+  "join_ballot a b s s' \<equiv>
+    let onebs'  = (finfun_acc_max_2 b) o$ ((op o$ (flip op$ a)) o$ (vote s))
     in
-      b > (ballot s $ a) 
+      b > (ballot s $ a)
       \<and> s' = s\<lparr>ballot := (ballot s)(a $:= b),
         onebs := (onebs s)(a $:= (onebs s $ a)(b $:= Some onebs')),
         leader := (ampr2_state.leader s)(a $:= False)\<rparr>"
+end 
+
+subsection {* Implementing the @{text acquire_leadership} action*}
+
+locale acquire_leadership = 
+  fixes onebs :: "'a \<Rightarrow>f bal \<Rightarrow>f (inst \<Rightarrow>f ('v\<times>bal) option) option"
+  fixes b :: bal
+begin
+  
+definition onebs' where "onebs' \<equiv> (\<lambda> ff1 . (\<lambda> off2 . the off2) o$ ff1) o$ onebs"
+
+definition votes_at_b where "votes_at_b \<equiv> ((flip finfun_apply) b) o$ onebs'"
+  
+definition fold_fun where "fold_fun a ff \<equiv> 
+  (case_prod union) o$ ($ option_as_set o$ (votes_at_b $ a), ff $)"
+
+definition inst_votes where "inst_votes q \<equiv>
+  Finite_Set.fold fold_fun (K$ {}) q"
+
+lemma inst_votes_code[code]:"inst_votes (set xs) = fold fold_fun xs (K$ {})"
+proof (induct xs)
+  case Nil
+  then show ?case by (auto simp add:inst_votes_def)
+next
+  case (Cons a xs)
+  interpret folding_idem "fold_fun" "K$ {}"
+    apply (unfold_locales)
+    by (auto simp add:fun_eq_iff expand_finfun_eq fold_fun_def)
+  show ?case using insert_idem
+    by (metis (mono_tags, lifting) Cons.hyps List.finite_set comp_fun_commute eq_fold fold_commute_apply fold_simps(2) list.simps(15) inst_votes_def) 
+qed
+
+definition maxs where "maxs q \<equiv> (flip max_by_key snd) o$ inst_votes q"
+
+definition the_suggestion :: "('v\<times>bal) set \<Rightarrow> 'v option" where "the_suggestion m \<equiv> 
+  if m = {} then None else Some (fst (the_elem m))"
+
+definition suggestion :: "nat \<Rightarrow>f nat \<Rightarrow>f 'v option \<Rightarrow> 'a set \<Rightarrow> nat \<Rightarrow>f nat \<Rightarrow>f 'v option" 
+  where "suggestion old q \<equiv> (\<lambda> (m, ff) . ff(b $:= the_suggestion m))
+    o$ ($ maxs q, old $)"
+  
+end
+
+global_interpretation al:acquire_leadership onebs b
+  for onebs b .
+
+context ampr2_ioa
+begin
 
 definition acquire_leadership where
-  "acquire_leadership a q s s' \<equiv> let b = ballot s $ a in 
-    leading b = a
+  "acquire_leadership a q (s::('v,'a,'l) ampr2_state) s' \<equiv> let b = ballot s $ a in
+    leader b = a
     \<and> q \<in> quorums
     \<and> \<not> ampr2_state.leader s $ a 
-    \<and> (\<forall> a \<in> q . onebs s $ a $ b \<noteq> None)
-    \<and> s' = s\<lparr>leader := (ampr2_state.leader s)(a $:= True), 
-        suggestion := \<lambda> i . (suggestion s i)(b $:=
-          let m = distributed_safe_at.max_pair q (\<lambda> a . (the (onebs s $ a $ b)) i) in
-            map_option fst m)\<rparr>"
+    \<and> (\<forall> a \<in> q . ampr2_state.onebs s $ a $ b \<noteq> None)
+    \<and> s' = s\<lparr>leader := (ampr2_state.leader s)(a $:= True),
+        suggestion := al.suggestion (onebs s) b (suggestion s) q\<rparr>"
 
+subsection {* suggest and @{text do_vote}. *}
+  
 definition suggest where "suggest a i b v s s' \<equiv>
           v \<in> propCmd s
         \<and> ballot s $ a = b
         \<and> ampr2_state.leader s $ a
-        \<and> (suggestion s i) $ b = None
-        \<and> s' = s\<lparr>suggestion := (suggestion s)(i := (suggestion s i)(b $:= Some v))\<rparr>"
+        \<and> (suggestion s $ i) $ b = None
+        \<and> s' = s\<lparr>suggestion := (suggestion s)(i $:= (suggestion s $ i)(b $:= Some v))\<rparr>"
 
 definition do_vote where
   "do_vote a i v s s' \<equiv> let b = ballot s $ a in
-          vote s $ a $ i $ b = None
-        \<and> (suggestion s i) $ b = Some v
-        \<and> s' = s\<lparr>vote := (vote s)(a $:= (vote s $ a)(i $:= (vote s $ a $ i)(b $:= Some v)))\<rparr>"
+          vote s $ i $ b $ a = None
+        \<and> (suggestion s $ i) $ b = Some v
+        \<and> s' = s\<lparr>vote := (vote s)(i $:= (vote s $ i)(b $:= (vote s $ i $ b)(a $:= Some v)))\<rparr>"
 
-abbreviation chosen where
-  "chosen s i v \<equiv> ballot_array.chosen quorums (\<lambda> a b. vote s $ a $ i $ b) v"
+end 
+
+experiment begin
+
+text {* Proving a code equation for that seems tough... *}
+
+definition flip_binary_finfun :: "'a \<Rightarrow>f 'b \<Rightarrow>f 'c \<Rightarrow> 'b \<Rightarrow>f 'a \<Rightarrow>f 'c" where
+  "flip_binary_finfun ff \<equiv> Abs_finfun (\<lambda> b . Abs_finfun (\<lambda> a . (ff $ a $ b)))"
+  
+lift_definition flip_binary_finfun_2 :: "'a \<Rightarrow>f 'b \<Rightarrow>f 'c \<Rightarrow> 'b \<Rightarrow>f 'a \<Rightarrow>f 'c"
+  is "\<lambda> f . \<lambda> x y . f y x" oops
+  
+end 
+
+subsection {* The learn action. *}
+
+locale chosen_imp =
+  fixes vote :: "inst \<Rightarrow>f bal \<Rightarrow>f 'a \<Rightarrow>f 'v option"
+  and i :: inst
+  (* and q :: "'a set" *)
+  and v :: 'v
+begin
+
+definition at_i :: "bal \<Rightarrow>f 'a \<Rightarrow>f 'v option" where
+  "at_i \<equiv> vote $ i"
+  
+definition decision_at_bal where "decision_at_bal \<equiv>
+  (finfun_All o (op o$ (op= (Some v)))) o$ at_i"
+  -- {* TODO: forall in quorum! *}
+  
+definition chosen where "chosen \<equiv> finfun_Ex decision_at_bal"
+  
+end
+
+global_interpretation ci:chosen_imp vote i v for vote::"inst \<Rightarrow>f bal \<Rightarrow>f 'a \<Rightarrow>f 'v option" 
+  and i and v::'v .
+term ci.chosen
+  -- {* TODO: How to get rid of the type parameters? *}
+
+context ampr2_ioa
+begin
 
 definition learn where
-  "learn l i v s s' \<equiv> chosen s i v \<and> s' = s\<lparr>learned := (learned s)(l $:= (learned s $ l)(i $:= Some v))\<rparr>"
+  "learn l i v s s' \<equiv> ci.chosen TYPE('a) TYPE('b) (vote s) i v 
+    \<and> s' = s\<lparr>learned := (learned s)(l $:= (learned s $ l)(i $:= Some v))\<rparr>"
+
+subsection {* catch_up and the full transition relation. *}
 
 definition catch_up where
   "catch_up l1 l2 i v s s' \<equiv> learned s $ l2 $ i = Some v
     \<and> s' = s\<lparr>learned := (learned s)(l1 $:= (learned s $ l1)(i $:= Some v))\<rparr>"
 
 fun trans_rel where
-  "trans_rel r (ampr1.Propose c) r' = propose c r r'"
-| "trans_rel r ampr1.Internal r' = (
+  "trans_rel r (Propose c) r' = propose c r r'"
+| "trans_rel r Internal r' = (
     (\<exists> a b . join_ballot a b r r')
     \<or> (\<exists> a i v . do_vote a i v r r')
     \<or> (\<exists> a i b v . suggest a i b v r r')
     \<or> (\<exists> l1 l2 i v . catch_up l1 l2 i v r r')
     \<or> (\<exists> a q . acquire_leadership a q r r'))"
-| "trans_rel r (ampr1.Learn i v l) r' = learn l i v r r'"
+  | "trans_rel r (Learn i v) r' = (\<exists> l . learn l i v r r')"
 
 lemma trans_cases[consumes 1]:
   assumes "trans_rel r a r'"
@@ -105,19 +229,21 @@ lemma trans_cases[consumes 1]:
 | (suggest) a i b v where "suggest a i b v r r'"
 | (catch_up) l1 l2 i v where "catch_up l1 l2 i v r r'"
 | (acquire) a q where "acquire_leadership a q r r'"
-using assms by induct auto
+  using assms apply induct apply (simp add:learn_def)
+  by (metis assms learn paxos_action.exhaust trans_rel.simps(1) trans_rel.simps(2) trans_rel.simps(3)) 
 
 lemma trans_cases_2[consumes 1]:
   assumes "trans_rel r aa r'"
   obtains 
-  (propose) c where "propose c r r'" and "aa = ampr1.amp_action.Propose c"
-| (learn) l i v where "learn l i v r r'" and "aa = ampr1.amp_action.Learn i v l"
-| (join_ballot) a b where "join_ballot a b r r'" and "aa = ampr1.amp_action.Internal"
-| (do_vote) a i v where "do_vote a i v r r'" and "aa = ampr1.amp_action.Internal"
-| (suggest) a i b v where "suggest a i b v r r'" and "aa = ampr1.amp_action.Internal"
-| (catch_up) l1 l2 i v where "catch_up l1 l2 i v r r'" and "aa = ampr1.amp_action.Internal"
-| (acquire) a q where "acquire_leadership a q r r'" and "aa = ampr1.amp_action.Internal"
-using assms by induct auto
+  (propose) c where "propose c r r'" and "aa = Propose c"
+| (learn) l i v where "learn l i v r r'" and "aa = Learn i v"
+| (join_ballot) a b where "join_ballot a b r r'" and "aa = Internal"
+| (do_vote) a i v where "do_vote a i v r r'" and "aa = Internal"
+| (suggest) a i b v where "suggest a i b v r r'" and "aa = Internal"
+| (catch_up) l1 l2 i v where "catch_up l1 l2 i v r r'" and "aa = Internal"
+| (acquire) a q where "acquire_leadership a q r r'" and "aa = Internal"
+  using assms apply induct apply (simp add:learn_def)
+  by (metis assms learn paxos_action.exhaust trans_rel.simps(1) trans_rel.simps(2) trans_rel.simps(3)) 
 
 definition trans where
   "trans \<equiv> { (r,a,r') . trans_rel r a r'}"
@@ -125,7 +251,7 @@ definition trans where
 subsection {* The I/O-automaton *}
 
 definition ioa where
-  "ioa \<equiv> \<lparr>ioa.asig = asig, start = start, trans = trans\<rparr>"
+  "ioa \<equiv> \<lparr>ioa.asig = paxos_asig, start = start, trans = trans\<rparr>"
 
 lemmas simps = ioa_def asig_def start_def trans_def propose_def join_ballot_def 
   do_vote_def learn_def suggest_def catch_up_def acquire_leadership_def
