Isabelle2/AbstractMultiPaxosR2Code.thy
@@ -1,5 +1,5 @@
 theory AbstractMultiPaxosR2Code
-imports AbstractMultiPaxosR2 "~~/src/HOL/Library/FinFun_Syntax"
+imports AbstractMultiPaxosR2
 begin
 
 definition n :: nat where "n \<equiv> 3"
@@ -10,18 +10,26 @@ definition accs where "accs \<equiv> {1..n}"
 
 definition leader where "leader (b::nat) \<equiv> (b mod n) + 1"
                       
-global_interpretation card_quorums accs 
-  defines qs = "quorums" and num_accs = "nas"
-  -- {* @{term num_accs} is there just for code generation *}
+global_interpretation cq:card_quorums accs
+  defines qs = "cq.quorums" and nas = "cq.nas"
 apply (unfold_locales)
 apply (simp add: accs_def n_def)
 apply (simp add: accs_def)
 done
 
 global_interpretation ampr2_ioa qs leader
-  defines ampr2_start = start .
+  defines ampr2_start = start
+  and ampr2_join_ballot = join_ballot
+  and ampr2_acquire_leadership = acquire_leadership
+  and ampr2_suggest = suggest
+  and ampr2_do_vote = do_vote
+  and ampr2_learn = learn
+  and ampr2_catch_up = catch_up
+  .
 
-export_code ampr2_start in SML
+export_code ampr2_start propose acc_max join_ballot
+  ampr2_join_ballot ampr2_acquire_leadership
+  ampr2_suggest ampr2_do_vote learn catch_up in Scala
 
 value "ampr2_start::(nat, nat, nat) ampr2_state set"
 
