Isabelle2/AbstractMultiPaxosR2Correctness.thy
@@ -1,104 +1,32 @@
 theory AbstractMultiPaxosR2Correctness
-imports AbstractMultiPaxosR1 AbstractMultiPaxosR2 "../../IO-Automata/Simulations"
+imports AbstractMultiPaxosR1 AbstractMultiPaxosR2 Simulations
 begin
 
-print_locale ampr2_ioa
-
-locale ampr2_proof = IOA + quorums quorums + ampr2_ioa quorums for
-     quorums :: "'a set set" +
-  fixes ampr2_ioa :: "(('v,'a,'l)ampr2_state, ('v,'a,'l)ampr1.amp_action) ioa"
-  and ampr1_ioa :: "(('v,'a,'l)amp_state, ('v,'a,'l)ampr1.amp_action) ioa"
-  defines "ampr2_ioa \<equiv> ioa" and "ampr1_ioa \<equiv> ampr1.amp_ioa"
+locale ampr2_proof = IOA + quorums quorums + ampr2_ioa quorums leader 
+  + r1:ampr1_ioa quorums leader
+  for quorums :: "'a set set" and leader :: "bal \<Rightarrow> 'a" + 
+  fixes ampr2_ioa :: "(('v, 'a, 'l) ampr2_state, 'v paxos_action) ioa"
+    and ampr1_ioa :: "(('v, 'a, 'l) ampr1_state, 'v paxos_action) ioa"
+  defines "ampr2_ioa \<equiv> ioa" and "ampr1_ioa \<equiv> r1.ioa"
 begin
 
-definition ref_map :: "('v,'a,'l)ampr2_state \<Rightarrow> ('v,'a,'l)amp_state" where 
-  "ref_map s \<equiv> \<lparr> amp_state.propCmd = (propCmd s),
-  ballot = (\<lambda>a. ((ballot s) $ a)),
-  vote = (\<lambda>a i b. (vote s $ a $ i $ b)),
-  suggestion = (\<lambda>i b. ((suggestion s i) $ b)),
-  onebs = (\<lambda>a b. (onebs s $ a $ b)),
-  learned = (\<lambda>l i. (learned s $ l $ i)),
-  leader = (\<lambda>a. (ampr2_state.leader s $ a)) \<rparr>"
+definition ref_map where "ref_map s \<equiv> \<lparr>
+  ampr1_state.propCmd = propCmd s,
+  ampr1_state.ballot = ballot s,
+  ampr1_state.vote = (\<lambda> i a . vote s $ a $ i),
+  ampr1_state.suggestion = suggestion s,
+  ampr1_state.onebs = onebs s,
+  ampr1_state.leader = ampr2_state.leader s\<rparr>"
 
 term "ampr1_ioa"
 term "ampr2_ioa"
-
-lemma aux_proof:"(op $ (K$ False)(leading b $:= True)) = (\<lambda> a . leading b = a)"
-proof
-  fix a
-  have "(K$  False)(leading b $:= True) $ a = (leading b = a)"
-  proof(cases "leading b = a")
-    case True
-      thus ?thesis by (simp add: finfun_upd_apply_same)
-  next
-    case False
-      thus ?thesis by (simp add: finfun_upd_apply)
-  qed
-  thus "\<And>a. (K$  False)(leading b $:= True) $ a = (leading b = a)" by (simp add: finfun_upd_apply)
-qed
-
-lemma aux_proof1:"\<And>l i v b q. \<lbrakk>q \<in> quorums; \<forall>a \<in> q. ampr2_state.vote s $ a $ i $ b = Some v\<rbrakk> \<Longrightarrow>
-    (\<lambda>la. op $ ((ampr2_state.learned s)(l $:= (ampr2_state.learned s $ l)(i $:= Some v)) $ la)) = 
-      (\<lambda>l. op $ (ampr2_state.learned s $ l))(l := op $ (ampr2_state.learned s $ l) (i \<mapsto> v))"
-proof
-  fix l i v b q la
-  assume 0:"q \<in> quorums" and 1:"\<forall>a \<in> q. ampr2_state.vote s $ a $ i $ b = Some v"
-  let ?t = "op $ ((ampr2_state.learned s)(l $:= (ampr2_state.learned  s $ l)(i $:= Some v)) $ la) =
-    ((\<lambda>l. op $ (ampr2_state.learned s $ l)) (l := op $ (ampr2_state.learned s $ l) (i \<mapsto> v))) la"
-  have ?t
-  proof(cases ?t)
-    case True
-      thus ?thesis by metis
-  next
-    case False
-      thus ?thesis by (metis (no_types, lifting) finfun_update.rep_eq fun_upd_def)
-  qed
-  thus ?t by blast
-qed
-
-lemma aux_proof2:"\<lbrakk>b = ampr2_state.ballot s $ a; ampr2_state.suggestion s i $ b = None\<rbrakk> \<Longrightarrow>
-  (\<lambda>ia. op $ (if ia = i then (ampr2_state.suggestion s i)(b $:= Some v) else ampr2_state.suggestion s ia)) =
-    (\<lambda>i. op $ (ampr2_state.suggestion s i))(i := op $ (ampr2_state.suggestion s i) (b \<mapsto> v))"
-proof
-  fix ia
-  assume "b = ampr2_state.ballot s $ a" and "ampr2_state.suggestion s i $ b = None"
-  let ?t = "op $ (if ia = i then (ampr2_state.suggestion s i)(b $:= Some v) else ampr2_state.suggestion s ia) =
-    ((\<lambda>i. op $ (ampr2_state.suggestion s i))(i := op $ (ampr2_state.suggestion s i)(b \<mapsto> v))) ia"
-  have ?t
-  proof(cases ?t)
-    case True
-      thus ?thesis by metis
-  next
-    case False
-      thus ?thesis by (smt finfun_update.rep_eq fun_upd_apply)
-  qed
-  thus ?t by blast
-qed
-
-lemma aux_proof3:"(\<lambda>l. op $ ((ampr2_state.learned s)(l1 $:= (ampr2_state.learned s $ l1)(i $:= Some v)) $ l)) =
-  (\<lambda>l. op $ (ampr2_state.learned s $ l))(l1 := op $ (ampr2_state.learned s $ l1)(i \<mapsto> v))"
-proof
-  fix l
-  let ?t = "op $ ((ampr2_state.learned s)(l1 $:= (ampr2_state.learned s $ l1)(i $:= Some v)) $ l) =
-    ((\<lambda>l. op $ (ampr2_state.learned s $ l))(l1 := op $ (ampr2_state.learned s $ l1)(i \<mapsto> v))) l"
-  have ?t
-  proof(cases ?t)
-    case True
-      thus ?thesis by blast
-  next
-    case False
-      thus ?thesis by auto
-  qed
-  thus "\<And>l. ?t" by blast
-qed
-  
 
 lemma "is_ref_map ref_map ampr2_ioa ampr1_ioa"
 proof (auto simp add:is_ref_map_def simp del:split_paired_Ex)
   fix s
   assume "s \<in> ioa.start ampr2_ioa"
   thus "ref_map s \<in> ioa.start ampr1_ioa" 
-    by (simp add:ref_map_def ampr2_ioa_def ampr1_ioa_def ioa_def start_def ampr1.simps aux_proof)
+    by (simp add:ref_map_def ampr1.simps ampr2_ioa_def ampr1_ioa_def ioa_def start_def)
 next
   fix s t a
   assume a1:"reachable ampr2_ioa s" and a2:"s \<midarrow>a\<midarrow>ampr2_ioa\<longrightarrow> t"
@@ -107,21 +35,12 @@ next
   proof (auto simp add:refines_def ioa_simps trace_match_def trace_def schedule_def filter_act_def)
     show "(ref_map s, a, ref_map t) \<in> ioa.trans ampr1_ioa" using a2
     apply (simp add:ampr2_ioa_def ioa_def is_trans_def trans_def)
-    apply (simp add:ampr1_ioa_def ampr1.amp_ioa_def ampr1.amp_trans_def)
+    apply (simp add:ampr1_ioa_def ampr1.ioa_def ampr1.trans_def)
     apply (induct rule:trans_cases_2)
-    (* propose *)
-    apply (simp add:simps ampr1.simps ref_map_def)
-    (* learn *)
-    apply (simp add:simps ampr1.simps ref_map_def ballot_array.chosen_def ballot_array.chosen_at_def)
-    apply (metis aux_proof1)
+    apply (simp_all add:simps ampr1.simps ref_map_def)[2]
     (* join_ballot *)
     apply (induct a) apply auto[2]
-    subgoal premises prems for a b
-    proof -
-      have "ampr1.join_ballot a b (ref_map s) (ref_map t)" using prems
-        by (auto simp add:ref_map_def simps Let_def ampr1.simps fun_eq_iff)
-      thus ?thesis by auto
-    qed
+    apply (auto simp add:ref_map_def ampr1.simps simps)[1]
     (* do_vote *)
     apply (induct a) apply auto[2] 
     subgoal premises prems for a i v
@@ -134,8 +53,8 @@ next
     apply (induct a) apply auto[2] 
     subgoal premises prems for a i b v
     proof -
-      have "ampr1.suggest a i b v (ref_map s) (ref_map t)" using prems(1)
-        by (auto simp add:suggest_def ampr1.suggest_def ref_map_def aux_proof2)
+      have "ampr1.suggest a i b v (ref_map s) (ref_map t)" using prems
+        by (auto simp add:ref_map_def simps Let_def ampr1.simps fun_eq_iff)
       thus ?thesis by auto
     qed
     (* catch_up *)
@@ -143,7 +62,7 @@ next
     subgoal premises prems for l1 l2 i v
     proof -
       have "ampr1.catch_up l1 l2 i v (ref_map s) (ref_map t)" using prems
-        by (auto simp add:catch_up_def ampr1.catch_up_def ref_map_def aux_proof3)
+        by (auto simp add:ref_map_def simps Let_def ampr1.simps fun_eq_iff)
       thus ?thesis by auto
     qed
     (* acquire_leadership *)
@@ -151,8 +70,7 @@ next
     subgoal premises prems for aa q
     proof -
       have "ampr1.acquire_leadership aa q (ref_map s) (ref_map t)" using prems
-        apply (auto simp add:acquire_leadership_def ampr1.acquire_leadership_def ref_map_def)
-        by (auto simp add:simps Let_def ampr1.simps fun_eq_iff)
+        by (auto simp add:ref_map_def simps Let_def ampr1.simps fun_eq_iff)
       thus ?thesis by auto
     qed
     done 
