Isabelle2/BallotArrayProperties.thy
@@ -1,18 +1,58 @@
 section {* Properties of ballot arrays. *}
 
 theory BallotArrayProperties
-imports Main BallotArrays Quorums 
+imports BallotArrays Quorums "~~/src/HOL/Library/Monad_Syntax"
 begin
 
+text {* 
+In this theory we show the two main properties of ballot-arrays:
+1) If a value v is @{term "ballot_array.proved_safe_at_abs q b v"}, then it is @{term "ballot_array.safe_at v b"}}
+2) If a ballot array increases, according to the prefix definition below, then every
+value that was @{term "ballot_array.safe_at v b"} before is still @{term "ballot_array.safe_at v b"}}}
+*}
+
 subsection {* Correctness of the @{term proved_safe_at} computation *}
+
+context ballot_array
+begin
+
+definition a_votes where "a_votes a bound \<equiv> {(v,b) . b < bound \<and> vote a b = Some v}"
+
+lemma a_votes_finite:
+  shows "finite (a_votes a bound)"
+proof - 
+  have 1:"finite (S \<bind> f)" if "finite S" and "\<And> x . x \<in> S \<Longrightarrow> finite (f x)" for S f
+    by (simp add: bind_UNION that)
+  have 2:"a_votes a bound = {b . b < bound} \<bind> (\<lambda> b . case vote a b of Some v \<Rightarrow> {(v,b)} | None  \<Rightarrow> {})"
+    (is "?votes = Set.bind ?bals ?f")
+    by (auto simp add: Set.bind_def a_votes_def split!:option.split)
+  have 3:"finite ?bals"
+    by simp 
+  have 4:"finite (?f b)" for b by (simp split!:option.split)
+  show ?thesis
+    by (metis (no_types, lifting) 2 3 1 4)
+qed
+
+definition q_votes where "q_votes q bound \<equiv> {(v,b) . b < bound \<and> (\<exists> a \<in> q . vote a b = Some v)}"
+
+end
 
 locale ballot_array_props = ballot_array quorums + quorums quorums for quorums
 begin
 
+lemma q_votes_q_votes:
+  "q_votes q bound = (\<Union> a\<in>q . a_votes a bound)"
+    by (auto simp add:q_votes_def a_votes_def)
+  
+lemma q_votes_finite:
+  assumes "q \<in> quorums"
+  shows "finite (q_votes q bound)" using assms(1) a_votes_finite quorums_axioms
+  by (auto simp add:a_votes_def q_votes_q_votes quorums_def)
+  
 context 
 begin 
 
-lemma "safe_at v (bot::nat)"
+lemma safe_at_0:"safe_at v (0::nat)"
 by (auto simp add:safe_at_def)
 
 (* Only used in safe \<Rightarrow> agreement *)
@@ -75,52 +115,57 @@ proof -
   show ?thesis using chosen_at_same 1 2 by (metis linorder_neqE_nat)
 qed
 
+subsection {* Proof that the proved_safe_at computation is correct. *}
+
+lemma proved_safe_at_cases:
+  assumes "proved_safe_at_abs q i v"
+    -- {* There are two cases: 
+    (a) an acceptor a in the quorum q voted in round k < i, 
+    and k is the maximum round smaller than i in which an acceptor in q voted;
+    (b) no acceptor in the quorum q voted in any round k < i *}
+  obtains 
+    (a) k a
+  where "a \<in> q" and "vote a k = Some v" and "k < i"
+    and "\<And> a\<^sub>2 l . \<lbrakk>a\<^sub>2 \<in> q; k < l; l < i\<rbrakk> \<Longrightarrow> vote a\<^sub>2 l = None"
+  | (b) "\<And> a k . \<lbrakk>a \<in> q; k < i\<rbrakk>  \<Longrightarrow> vote a k = None"
+proof -
+  have "q \<in> quorums" and ballot_q:"\<And> a . a \<in> q \<Longrightarrow> ballot a \<ge> i" 
+    using \<open>proved_safe_at_abs q i v\<close> by (auto simp add:proved_safe_at_abs_def)
+  show ?thesis 
+  proof (cases "\<exists> a \<in> q . \<exists> l . l < i \<and> vote a l \<noteq> None")
+    case False thus ?thesis using that by blast
+  next
+    case True
+    let ?votes="{(w,m) . m < i \<and> (\<exists> a \<in> q . vote a m = Some w)}"
+    have 1:"v \<in> (fst ` (max_by_key ?votes snd))"  using True \<open>proved_safe_at_abs q i v\<close>
+      by (simp add:proved_safe_at_abs_def)
+    with this obtain x where 4:"x \<in> max_by_key ?votes snd" and 5:"fst x = v" by blast
+    have 2:"finite ?votes" using \<open>q \<in> quorums\<close> q_votes_finite
+      by (simp add: q_votes_def) 
+    have 3:"?votes \<noteq> {}" using True by auto 
+    have 6:"\<And> a\<^sub>2 l . \<lbrakk>a\<^sub>2 \<in> q; snd x < l; l < i\<rbrakk> \<Longrightarrow> vote a\<^sub>2 l = None" and 9:"snd x < i"
+      using 4 3 apply (auto simp add:max_by_key[OF 2, of snd]) by (meson not_le option.exhaust)
+    obtain a where 7:"a \<in> q" and 8:"vote a (snd x) = Some v" using \<open>x \<in> max_by_key ?votes snd\<close> 5
+      by (auto simp add:max_by_key[OF 2, of snd])
+    show ?thesis using that using 5 7 8 9 6 by auto
+  qed
+qed
+
 text {* The main lemma. Inspired by section 2.2.2 of the paper "Fast Paxos", by Leslie Lamport. *}
 
-lemma proved_safe_at_2_a_imp_safe_at:
+lemma proved_safe_at_abs_imp_safe_at:
   assumes "\<And> a j w . \<lbrakk>j < i; vote a j = Some w\<rbrakk> \<Longrightarrow> safe_at w j"
-  and "proved_safe_at_2_a q i v" and "conservative_array"
+  and "proved_safe_at_abs q i v" and "conservative_array"
   shows "safe_at v (i::nat)"
 proof (cases "i = 0")
   case True thus ?thesis
     by (metis not_less0 safe_at_def)
 next
   case False
-  have "q \<in> quorums" and ballot_q:"\<And> a . a \<in> q \<Longrightarrow> ballot a \<ge> i" using assms(2) by (auto simp add:proved_safe_at_2_a_def)
-  text {* There are two cases: 
-    (a) an acceptor a in the quorum q voted in round k < i, 
-    and k is the maximum round smaller than i in which an acceptor in q voted;
-    (b) no acceptor in the quorum q voted in any round k < i 
-    TODO: turn this into a lemma? *}
-  consider
-    (a) k a
-      where "a \<in> q" and "vote a k = Some v" and "k < i"
-      and "\<And> a\<^sub>2 l . \<lbrakk>a\<^sub>2 \<in> q; k < l; l < i\<rbrakk> \<Longrightarrow> vote a\<^sub>2 l = None"
-  | (b) "\<And> a k . \<lbrakk>a \<in> q; k < i\<rbrakk>  \<Longrightarrow> vote a k = None" 
-  proof (cases "\<exists> a \<in> q . \<exists> l . l < i \<and> vote a l \<noteq> None")
-    case False thus ?thesis using that by blast
-  next
-    case True
-    def votes \<equiv> "{l . \<exists> a \<in> q . l < i \<and> vote a l \<noteq> None }"
-    def k \<equiv> "Max votes"
-    from True assms(2) obtain a where "a \<in> q" and "vote a k = Some v"
-      by (auto simp add:proved_safe_at_2_a_def k_def votes_def)
-    moreover have "k < i" and "\<And> a\<^sub>2 l . \<lbrakk>a\<^sub>2 \<in> q; k < l; l < i\<rbrakk> \<Longrightarrow> vote a\<^sub>2 l = None"
-    proof -
-      have "k \<in> votes" and "\<And> x . x \<in> votes \<Longrightarrow> x \<le> k"
-      proof -
-        have "finite votes" and "votes \<noteq> {}" using True
-          using True votes_def finite_nat_set_iff_bounded votes_def by auto
-        thus "k \<in> votes" and "\<And> x . x \<in> votes \<Longrightarrow> x \<le> k" by (metis Max_in k_def, metis Max_ge k_def)
-      qed
-      thus "k < i" and "\<And> a\<^sub>2 l . \<lbrakk>a\<^sub>2 \<in> q; k < l; l < i\<rbrakk> \<Longrightarrow> vote a\<^sub>2 l = None" 
-        by (force simp add:votes_def)+
-    qed
-    ultimately show ?thesis using that by blast
-  qed
-  text {* now we prove the thesis by considering the cases (a) and (b) separately *}
-  thus ?thesis
-  proof (cases)
+  have "q \<in> quorums" and ballot_q:"\<And> a . a \<in> q \<Longrightarrow> ballot a \<ge> i" 
+    using \<open>proved_safe_at_abs q i v\<close> by (auto simp add:proved_safe_at_abs_def)
+  show ?thesis using \<open>proved_safe_at_abs q i v\<close>
+  proof (cases rule:proved_safe_at_cases)
     case b
     text {* We prove that no value is choosable at any @{text "j < i"}; 
       therefore, anything is safe at i *}
@@ -136,7 +181,7 @@ next
       ultimately have False by auto }
     thus "safe_at v i" by (auto simp add:safe_at_def)
   next
-    case a
+    case (a k a)
     have "v' = v" if "choosable v' j" and "j < i" for j v'
     proof -
       text {* First obtain an acceptor that has voted for v' in j *}
@@ -168,7 +213,7 @@ next
       next
         case bb
         with \<open>conservative_array\<close> \<open>vote a2 j = Some v'\<close> \<open>vote a k = Some v\<close> show ?thesis 
-          by (simp add:conservative_def conservative_array_def split add:option.splits)
+          by (simp add:conservative_def conservative_array_def split: option.splits)
       qed
     qed
     thus ?thesis by (metis safe_at_def)
@@ -188,7 +233,7 @@ definition is_prefix where
   "is_prefix b1 b2 v1 v2 \<equiv> \<forall> a . b1 a \<le> b2 a 
     \<and> (\<forall> b . (b < b1 a \<or> (b = b1 a \<and> v1 a b \<noteq> None)) \<longrightarrow> v1 a b = v2 a b)"
 
-locale ballot_array_prefix = quorums quorums for quorums :: "'a set set" +
+locale ballot_array_prefix = quorums quorums for  quorums :: "'a set set" +
   -- {* @{typ 'a} is the type of acceptors *}
   fixes ballot1 :: "'a \<Rightarrow> nat"
   and vote1 :: "'a \<Rightarrow> nat \<Rightarrow> 'v option"
@@ -215,11 +260,18 @@ lemma safe_at_mono:
   shows "ba_2.safe_at v b"
   by (metis assms ba_1.safe_at_def ba_2.safe_at_def choosable_decreases)
 
+lemma chosen_mono:
+  assumes "ba_1.chosen v" and "ba_1.well_formed"
+  shows "ba_2.chosen v" using assms ballot_array_prefix_axioms
+  unfolding ba_1.chosen_def ba_2.chosen_def ballot_array_prefix_def quorums_def ballot_array_prefix_axioms_def
+    is_prefix_def ba_2.chosen_at_def ba_1.chosen_at_def ba_1.well_formed_def apply auto
+  by (metis not_less_iff_gr_or_eq option.distinct(1))
+  
 lemma safe_votes:
   assumes ba_1.safe and "\<And> b a v . \<lbrakk>vote1 a b \<noteq> vote2 a b; vote2 a b = Some v\<rbrakk> \<Longrightarrow> ba_1.safe_at v b"
   and "\<And> b a . b > ballot1 a \<Longrightarrow> vote1 a b = vote2 a b"
   shows ba_2.safe
-proof (auto simp add:ballot_array.safe_def split add:option.splits)
+proof (auto simp add:ballot_array.safe_def split:option.splits)
   fix a b v
   assume "vote2 a b = Some v"
   show "ba_2.safe_at v b"
