Isabelle2/DistributedSafeAt.thy
@@ -1,177 +1,111 @@
 theory DistributedSafeAt
-imports BallotArrays BallotArrayProperties
+imports BallotArrays BallotArrayProperties "~~/src/HOL/Library/Monad_Syntax" Utils
 begin
 
-subsection {* Computing safe values in a distributed implementation *}
-
-locale distributed_safe_at = ballot_array 
+section {* Computing safe values in a distributed implementation *}
+  
+locale distributed_safe_at = ballot_array
 begin
 
 definition acc_max where
   -- {* @{term acc_max} can be computed locally by an acceptor. *}
-  "acc_max a bound \<equiv> 
-    if (\<exists> b < bound . vote a b \<noteq> None)
-    then Some (the_elem (max_by_key_2 {(v,b) . b < bound \<and> vote a b = Some v} snd))
-    else None"
-
-definition max_pair where
-  "max_pair q a_max \<equiv> 
-    let acc_maxs = Union ((\<lambda> a . case a_max a of None \<Rightarrow> {} | Some (v,b) \<Rightarrow> {(v,b)}) ` q)
-    in
-      if acc_maxs = {} then None
-      else Some (max_by_key_2 acc_maxs snd)"
+  "acc_max a bound \<equiv> max_by_key (a_votes a bound) snd"
+  
+definition max_quorum_votes where
+  "max_quorum_votes q b \<equiv> max_by_key (\<Union> a \<in> q . acc_max a b) snd"
 
 definition proved_safe_at where
-  -- {* @{term proved_safe_at} can be computed locally by a leader *}
+  -- {* @{term proved_safe_at} can be computed locally by a leader when it knows acc_max over q *}
   "proved_safe_at q b v \<equiv> q \<in> quorums \<and> (\<forall> a \<in> q . ballot a \<ge> b) \<and>
-    (case max_pair q (\<lambda> a . acc_max a b) of None \<Rightarrow> True
-    | Some S \<Rightarrow> v \<in> (fst ` S))"
-          
-end
-
-print_locale distributed_safe_at
-print_locale quorums
-
-locale dsa_properties = quorums quorums + distributed_safe_at quorums for quorums
-begin
-
-context begin
-                                                         
-private     
-
-lemma l0: assumes "\<exists> b < bound . vote a b \<noteq> None" and "S = {(v, b). b < bound \<and> vote a b = Some v}" and "finite S"
-  shows "card (max_by_key_2 S snd) = 1"
-unfolding max_by_key_2_def
-proof-
-  have 0:"S \<noteq> {}" using assms(1,2)
-    using Collect_empty_eq case_prodI not_Some_eq by blast
-  obtain b' where 1:"b' = Max (snd ` S)" by simp
-  with this obtain v' where 2:"vote a b' = Some v'" using assms(1,2,3) 0
-    by (smt Max_in Product_Type.Collect_case_prodD finite_imageI imageE image_is_empty)
-  hence 3:"(v', b') \<in> {x \<in> S. snd x = Max (snd ` S)}" using "0" "1" "2" assms(2) assms(3) by auto
-  {
-    assume "\<exists>(v'',b'') \<in> {x \<in> S. snd x = Max (snd ` S)}. (v'',b'') \<noteq> (v', b')"
-    hence "False" using 2 by (simp add: "1" assms(2) case_prodE eq_snd_iff mem_Collect_eq option.inject)
-  }
-  hence "{x \<in> S. snd x = Max (snd ` S)} = {(v', b')}" using "3" by blast
-  thus "card {x \<in> S. snd x = Max (snd ` S)} = 1" by simp
-qed
-  
-                                             
-lemma l1: assumes "proved_safe_at q b v" and "conservative_array"
-  shows "proved_safe_at_2_a q b v"
-proof -
-  text {* First a few immediate facts. *}
-  from assms have "q \<in> quorums" and bals:"\<And> a . a \<in> q \<Longrightarrow> ballot a \<ge> b" using proved_safe_at_def
-    apply force by (meson assms(1) proved_safe_at_def)
-  from \<open>q \<in> quorums\<close> have "finite q" and "q \<noteq> {}"
-    apply (metis quorums_axioms quorums_def) by (metis \<open>q \<in> quorums\<close> empty_iff quorum_inter_witness)
-
-  text {* Re-stating the main goal. *}
-  have "if \<exists> a \<in> q . \<exists> b\<^sub>2 . b\<^sub>2 < b \<and> vote a b\<^sub>2 \<noteq> None
-    then \<exists> a \<in> q . vote a (Max {b\<^sub>2 . \<exists> a \<in> q . b\<^sub>2 < b \<and> vote a b\<^sub>2 \<noteq> None}) = Some v
-    else True" (is "if ?cond then ?true else ?false")
-  proof (cases "?cond")
-    case True    
-    from True obtain a b\<^sub>a where t0:"a \<in> q" and t1:"vote a b\<^sub>a \<noteq> None" and t2:"b\<^sub>a < b" by (auto simp add:acc_max_def)
-    hence "acc_max a b \<noteq> None" by (auto simp add:acc_max_def)
-
-    text {* Using lemma @{thm max_by_key_subsets} *}
-    let ?Ss = "{{(v,b\<^sub>a) . b\<^sub>a < b \<and> vote a b\<^sub>a = Some v} | a . a \<in> q}"
-    let ?S = "{(v,b\<^sub>a) . b\<^sub>a < b \<and> vote a b\<^sub>a = Some v}"
-    have 8:"finite ?Ss" using \<open>finite q\<close> by simp
-    have 9:"\<And> S . S \<in> ?Ss \<Longrightarrow> finite S"
-    proof -
-      { fix S f g
-        assume "finite (f ` S)" and "\<And> x . x \<in> S \<Longrightarrow> x = (g o f) x"
-        hence "finite S" by (metis finite_imageI finite_subset image_comp image_eqI subsetI) }
-      note 1 = this
-      fix S assume "S \<in> ?Ss"
-      obtain a where 2:"S = {(v,b\<^sub>a) . b\<^sub>a < b \<and> vote a b\<^sub>a = Some v}" by (smt \<open>S \<in> ?Ss\<close> mem_Collect_eq)
-      moreover with this have "\<And> x . x \<in> S \<Longrightarrow> x = (the (vote a (snd x)), snd x)" by (metis (mono_tags, lifting) Product_Type.Collect_case_prodD option.sel prod.collapse) 
-      moreover have "finite (snd ` S)" using 2 by (auto simp add:image_def)
-      ultimately show "finite S" using 1[of snd S "\<lambda> b . (the (vote a b), b)"] by (metis comp_def)
-    qed
-    have 5:"?S \<in> ?Ss" using \<open>a \<in> q\<close> by blast
-    have 6:"?S \<noteq> {}" using \<open>b\<^sub>a < b\<close> \<open>vote a b\<^sub>a \<noteq> None\<close> by blast
-    have v_max_max:"v \<in> fst ` (max_by_key_2 (Union {max_by_key_2 S snd | S . S \<in> ?Ss \<and> S \<noteq> {}}) snd)" 
-    proof -
-      let ?acc_maxs_set = "(\<lambda> a . case acc_max a b of None \<Rightarrow> {} | Some (v,b) \<Rightarrow> {(v,b)}) ` q"
-      let ?acc_maxs = "Union ?acc_maxs_set"
-      have 1:"?acc_maxs \<noteq> {}" using \<open>acc_max a b \<noteq> None\<close> apply (auto split add:option.splits) by (metis \<open>a \<in> q\<close>)
-      hence 2:"fst (max_by_key_2 ?acc_maxs snd) = v" using assms(1) proved_safe_at_def 
-        apply (auto simp add:max_pair_def split add:option.splits) 
-        apply (metis option.simps(3)) 
-        by (metis (no_types, lifting) fst_conv option.inject) 
-      moreover
-      have 7:"?acc_maxs = {max_by_key S snd | S . S \<in> ?Ss \<and> S \<noteq> {}}"
-        apply (auto simp add: acc_max_def split add:option.splits split_if_asm)
-        apply (smt Collect_empty_eq case_prodI) by (metis (mono_tags) option.simps(3))
-      ultimately show ?thesis by auto 
-    qed
-    hence v_max_Union:"v \<in> fst ` (max_by_key_2 (Union ?Ss) snd)"
-    proof -
-      have 10:"\<And> x y . \<lbrakk>x \<in> Union ?Ss; y \<in> Union ?Ss; snd x = snd y\<rbrakk> \<Longrightarrow> x = y"
-        using assms(2) by (auto simp add:conservative_array_def conservative_def split add:option.splits)
-      show ?thesis using max_by_key_2_subsets[of ?Ss ?S snd]
-        by (metis (no_types, lifting) "10" "5" "6" "8" "9" v_max_max) 
-    qed
-
-    text {* now we prove that this is the same as Max... *}
-    let ?m = "(max_by_key_2 (Union ?Ss) snd)"  let ?b\<^sub>m = "(snd ` ?m)"
-    have 13:"v \<in> fst ` ?m" by (metis v_max_Union)
-    let ?bals = "{b\<^sub>2 . b\<^sub>2 < b \<and> (\<exists> a \<in> q . vote a b\<^sub>2 \<noteq> None)}"
-    have bm_max:"Max ?bals \<in> ?b\<^sub>m" sorry
-    (*proof -
-      have "card (snd ` ?m) = 1"  using \<open>b\<^sub>a < b\<close> \<open>vote a b\<^sub>a \<noteq> None\<close> unfolding max_by_key_2_def 
-      have "?b\<^sub>m \<in> ?bals" and "\<And> b . b \<in> ?bals \<Longrightarrow> b \<le> ?b\<^sub>m"
-      proof -
-        have 14:"(v,?b\<^sub>m) \<in> Union ?Ss" and 15:"\<And> x . x \<in> Union ?Ss \<Longrightarrow> snd x \<le> ?b\<^sub>m" 
-        proof -
-          have 11:"finite (Union ?Ss)" by (metis (no_types, lifting) "8" "9" finite_Union)
-          have 12:"Union ?Ss \<noteq> {}" by (metis (no_types, lifting) "5" "6" Sup_bot_conv(1))
-          show "(v,?b\<^sub>m) \<in> Union ?Ss" and 15:"\<And> x . x \<in> Union ?Ss \<Longrightarrow> snd x \<le> ?b\<^sub>m"
-            
-        qed
-        have 18:"?b\<^sub>m < b" using 14 by auto 
-        have 16:"Union ?Ss = {(v\<^sub>2,b\<^sub>2) . b\<^sub>2 < b \<and> (\<exists> a \<in> q . vote a b\<^sub>2 = Some v\<^sub>2)}" by auto
-        have 17:"\<exists> a \<in> q . vote a ?b\<^sub>m = Some v" and 19:"\<And> b\<^sub>2 v\<^sub>2. b\<^sub>2 < b \<and> (\<exists> a \<in> q . vote a b\<^sub>2 = Some v\<^sub>2) \<Longrightarrow> b\<^sub>2 \<le> ?b\<^sub>m"
-          apply (smt "14" "16" Product_Type.Collect_case_prodD prod.collapse v_max_Union)
-          by (metis (mono_tags, lifting) "15" "16" case_prod_conv mem_Collect_eq snd_conv)
-        show "?b\<^sub>m \<in> ?bals" and "\<And> b . b \<in> ?bals \<Longrightarrow> b \<le> ?b\<^sub>m"
-          apply (metis (mono_tags, lifting) "17" "18" mem_Collect_eq option.simps(3))
-          apply auto apply (insert 19) by (metis (no_types, lifting)) 
-      qed
-      moreover have "finite ?bals" by fastforce
-      moreover have "?bals \<noteq> {}"
-        by (metis (mono_tags, lifting) Collect_empty_eq \<open>a \<in> q\<close> \<open>b\<^sub>a < b\<close> \<open>vote a b\<^sub>a \<noteq> None\<close>) 
-      ultimately show "?b\<^sub>m = Max ?bals" by (metis (no_types, lifting) Max_eqI)
-    qed*)
-    have m_in_union:"?m = Union ?Ss" 
-    proof -
-      have "finite (Union ?Ss)" by (metis (no_types, lifting) "8" "9" finite_Union) 
-      moreover have "Union ?Ss \<noteq> {}"
-        by (metis (mono_tags, lifting) "5" "6" empty_Union_conv)
-      ultimately show ?thesis sorry
-    qed
-    obtain a2 where "a2 \<in> q" and max_vote:"\<forall>b \<in> ?b\<^sub>m. vote a2 b = Some v" sorry
-      (*by (smt Product_Type.Collect_case_prodD UnionE m_in_union mem_Collect_eq v_max_Union) *)
-    show ?thesis using bexI[where ?x=a2 and ?A=q] max_vote True \<open>a2 \<in> q\<close> bm_max by auto
-  next
-    case False
-    thus ?thesis by auto
-  qed
-  thus ?thesis using \<open>q \<in> quorums\<close> bals by (auto simp add:proved_safe_at_2_a_def)
-qed
-
-lemma proved_safe_at_imp_safe_at:
-  assumes "\<And> a j w . \<lbrakk>j < i; vote a j = Some w\<rbrakk> \<Longrightarrow> safe_at w j"
-  and "proved_safe_at q i v" and "conservative_array"
-  shows "safe_at v (i::nat)" using l1 ballot_array_props.proved_safe_at_2_a_imp_safe_at
-by (metis assms(1) assms(2) assms(3) ballot_array_props.intro quorums_axioms) 
-
-end
+    (v \<in> (fst ` max_quorum_votes q b) \<or> max_quorum_votes q b = {})"
 
 end 
+
+subsection {* Properties of @{term distributed_safe_at.proved_safe_at} *}
+
+locale dsa_properties = quorums quorums + distributed_safe_at quorums ballot vote 
+  for quorums ballot vote
+begin
+
+sublocale ballot_array_props 
+  by (unfold_locales)
+
+context begin
+
+private
+lemma max_quorum_votes:
+  assumes "q \<in> quorums"
+  shows "max_quorum_votes q b =
+  max_by_key (q_votes q b) snd"
+  (is "?lhs = max_by_key ?vs snd")
+proof -
+  define Ss where "Ss \<equiv> {a_votes a b | a . a \<in> q}"
+  have "finite S" if "S \<in> Ss" for S using that using Ss_def a_votes_finite by blast 
+  moreover
+  have "finite Ss" using \<open>q \<in> quorums\<close> using  quorums_axioms unfolding Ss_def quorums_def  by auto
+  moreover have "{(v, b'). b' < b \<and> (\<exists>a\<in>q. vote a b' = Some v)} = \<Union> Ss"
+    unfolding Ss_def a_votes_def by auto
+  moreover have "(\<Union>a\<in>q. acc_max a b) = (\<Union>S\<in>Ss . max_by_key S snd)" unfolding Ss_def acc_max_def by auto
+  ultimately show ?thesis using max_by_key_subsets[of Ss snd] unfolding max_quorum_votes_def q_votes_def by auto
+qed 
+ 
+lemma max_vote_e_or_singleton:
+  assumes "conservative_array" and "q \<in> quorums"
+  obtains x where "max_quorum_votes q b = {x}"
+  | "max_quorum_votes q b = {}"
+proof (cases "\<exists> a \<in> q . \<exists> b' < b . vote a b' \<noteq> None")
+  case True
+  define vs where "vs \<equiv> q_votes q b"
+  have "vs \<noteq> {}" using True unfolding vs_def q_votes_def by auto
+  moreover have "finite vs" unfolding vs_def
+    by (simp add: assms(2) q_votes_finite) 
+  moreover have "snd x \<noteq> snd y" if "x \<in> vs" and "y \<in> vs" and "x \<noteq> y" for x y 
+    using assms(1) that unfolding vs_def conservative_array_def conservative_def q_votes_def
+    by (auto split!:option.splits) 
+  moreover have "max_quorum_votes q b = max_by_key vs snd" unfolding vs_def q_votes_def
+    by (simp add:max_quorum_votes[OF assms(2)] q_votes_def)
+  ultimately
+  obtain x where "max_quorum_votes q b = {x}" using max_by_key_ordered by metis
+  thus ?thesis using that by auto
+next
+  case False
+  then show ?thesis using that max_quorum_votes[OF assms(2)] unfolding max_by_key_def q_votes_def by fastforce
+qed
+
+private lemma safe_at_imp_safe_at_abs:
+  assumes "proved_safe_at q b v" and "q \<in> quorums"
+  shows "proved_safe_at_abs q b v"
+proof (cases "max_quorum_votes q b = {}")
+  case True
+  hence "max_by_key (q_votes q b) snd = {}"  by (simp add:max_quorum_votes[OF \<open>q\<in>quorums\<close>])
+  moreover have "finite (q_votes q b)" by (simp add: assms(2) q_votes_finite) 
+  ultimately have "q_votes q b = {}" by (meson max_by_key_ne) 
+  hence "\<not> (\<exists> a \<in> q . \<exists> b' . b' < b \<and> vote a b' \<noteq> None)" 
+    apply (auto simp add:q_votes_def) by (meson option.exhaust)
+  then show ?thesis using assms by (auto simp add:proved_safe_at_abs_def proved_safe_at_def)
+next
+  case False
+  then show ?thesis 
+    using  assms unfolding proved_safe_at_def
+    by (auto simp add:max_quorum_votes[OF assms(2)] proved_safe_at_abs_def q_votes_def)
+qed
+
+private
+lemma proved_safe_at_imp_safe_at_aux:
+  assumes "\<And> a j w . \<lbrakk>j < i; vote a j = Some w\<rbrakk> \<Longrightarrow> safe_at w j"
+    and "proved_safe_at q i v" and "conservative_array" and "q \<in> quorums"
+  shows "safe_at v (i::nat)" using safe_at_imp_safe_at_abs assms proved_safe_at_abs_imp_safe_at
+  by blast
+
+lemma proved_safe_at_imp_safe_at:
+  -- {* A weaker version of the above, but which is easier to use in proofs. *}
+  assumes "safe"
+    and "proved_safe_at q i v" and "conservative_array" and "q \<in> quorums"
+  shows "safe_at v (i::nat)" using assms proved_safe_at_imp_safe_at_aux
+  by (metis option.simps(5) safe_def)
+  
+end
+
+end
 
 end
