Isabelle2/AbstractMultiPaxos.thy
@@ -1,0 +1,84 @@
+theory AbstractMultiPaxos
+imports  IOA BallotArrays Paxos_Sig
+begin                          
+
+section {* Definition of the Abstract MultiPaxos I/O-automaton *}
+
+subsection {* State and actions *}
+
+record ('v,'a) amp_state =
+  propCmd :: "'v set"
+  ballot :: "'a \<Rightarrow> nat"
+  vote :: "inst \<Rightarrow> 'a \<Rightarrow> bal \<Rightarrow> 'v option"
+  -- {* TODO: according to Isabelle's canonical argument order, 
+  it shoudl be @{typ "'a \<Rightarrow> bal \<Rightarrow> inst \<Rightarrow> 'v option"} *}
+
+locale amp_ioa =
+  fixes quorums::"'a set set"
+begin
+
+definition amp_start where
+  -- {* The initial state *}
+  "amp_start \<equiv> {\<lparr>propCmd = {}, ballot = (\<lambda> a . 0), vote = (\<lambda> i a b . None) \<rparr>}"
+
+subsection {* The transitions *}
+
+definition propose where
+  "propose c r r' \<equiv> (r' = r\<lparr>propCmd := (propCmd r) \<union> {c}\<rparr>)"
+
+definition join_ballot where
+  "join_ballot a b s s' \<equiv>
+    b > (ballot s a) \<and> s' = s\<lparr>ballot := (ballot s)(a := b)\<rparr>"
+
+abbreviation proved_safe_at where 
+  -- {* v is proved safe in instance i at ballot b by quorum q *}
+  "proved_safe_at s i q b v \<equiv> ballot_array.proved_safe_at_abs quorums (ballot s) (vote s i) q b v"
+
+abbreviation conservative_at where
+  "conservative_at s i \<equiv> ballot_array.conservative_array (vote s i)"
+
+definition do_vote where
+  "do_vote a i q v s s' \<equiv> let b = ballot s a in
+          v \<in> propCmd s
+        \<and> vote s i a b = None
+        \<and> proved_safe_at s i q b v
+        \<and> q \<in> quorums
+        \<and> conservative_at s' i
+        \<and> s' = s\<lparr>vote := (vote s)(i := (vote s i)(a := (vote s i a)(b := Some v)))\<rparr>"
+
+abbreviation chosen where
+  "chosen s i v \<equiv> ballot_array.chosen quorums (vote s i) v"
+
+definition learn where
+  "learn i v s s' \<equiv> chosen s i v \<and> s = s'"
+
+fun amp_trans_rel where
+  "amp_trans_rel r (Propose c) r' = propose c r r'"
+| "amp_trans_rel r Internal r' = (
+    (\<exists> a b . join_ballot a b r r')
+    \<or> (\<exists> a q i v . do_vote a i q v r r'))"
+| "amp_trans_rel r (Learn i v) r' = learn i v r r'"
+
+lemma trans_cases: assumes "amp_trans_rel r a r'"
+  obtains 
+  (propose) c where "propose c r r'"
+| (learn) i v where "learn i v r r'"
+| (join_ballot) a b where "join_ballot a b r r'"
+| (do_vote) a i q v where "do_vote a i q v r r'"
+  using assms apply induct apply auto
+  by (meson amp_trans_rel.elims(2)) 
+
+definition amp_trans where
+  "amp_trans \<equiv> { (r,a,r') . amp_trans_rel r a r'}"
+
+subsection {* The I/O-automaton *}
+
+definition amp_ioa where
+  "amp_ioa \<equiv> \<lparr>ioa.asig = paxos_asig, start = amp_start, trans = amp_trans\<rparr>"
+
+lemmas simps = amp_ioa_def paxos_asig_def amp_start_def amp_trans_def propose_def join_ballot_def 
+  do_vote_def learn_def
+
+end
+
+end
