Isabelle2/AbstractMultiPaxosCorrectness.thy
@@ -1,0 +1,114 @@
+section {* Proof of the agreement property of AbstractMultiPaxos. *}
+
+theory AbstractMultiPaxosCorrectness
+imports AbstractMultiPaxos IOA_Automation BallotArrayProperties 
+begin
+
+locale amp_proof = quorums quorums + amp_ioa quorums for quorums +
+  fixes the_ioa
+  defines "the_ioa \<equiv> amp_ioa"
+  -- {* Here we have to fix the constant @{term the_ioa} in order to fix all type variables.
+  Otherwise, there are problems in Eisbach when matching the same polymorphic constant appearing in several terms. *}
+begin
+
+interpretation IOA .
+
+subsection {* Automation setup and a few lemmas *}
+
+lemmas amp_ioa_defs =
+   is_trans_def actions_def amp_trans_def amp_start_def
+   externals_def amp_ioa_def the_ioa_def paxos_asig_def
+
+declare amp_ioa_defs[inv_proofs_defs]
+declare amp_ioa_def[inv_proofs_defs]
+
+declare propose_def[simp] join_ballot_def[simp] do_vote_def[simp]
+  learn_def[simp] Let_def[simp] if_split[split] if_split_asm[split]
+
+subsection {* @{term conservative_array}  is an inductive invariant *}
+
+declare ballot_array.conservative_array_def[inv_proofs_defs]
+
+abbreviation conservative_array where
+"conservative_array s \<equiv>  \<forall> i . conservative_at s i"
+
+lemma conservative_inductive:
+  "invariant the_ioa conservative_array"
+  apply (try_solve_inv2 case_thm:trans_cases inv_proofs_defs:inv_proofs_defs ballot_array.conservative_def invs:invs)
+  apply (case_tac a)
+  apply (auto simp add:inv_proofs_defs split:option.split_asm)
+done
+declare conservative_inductive[invs]
+
+subsection {* @{term safe} is inductive relative to @{term conservative_array}} *}
+
+text {* 
+We first prove that when the algorithm takes a step, the old state is a prefix
+of the new state. With this fact, we obtain that (1) a safe value remains safe after a step using the lemma @{thm ballot_array_prefix.safe_at_mono }.
+Then we prove that (2) when a vote is cast at a ballot b from a safe state, then the voted value is safe at b.
+Given those two facts, the inductiveness of safe follows.  *}
+
+abbreviation safe_at where "safe_at s i \<equiv> ballot_array.safe_at  quorums (ballot s) (vote s i)"
+
+lemma trans_imp_prefix_order:
+  assumes "s \<midarrow>a\<midarrow>the_ioa\<longrightarrow> t"
+  shows "is_prefix (ballot s) (ballot t) (vote s i) (vote t i)" using assms
+by (cases a) (auto simp add:is_prefix_def inv_proofs_defs split:option.split_asm)
+
+lemma safe_mono:
+  -- {* @{term safe_at} is monotonic. *}
+  assumes "s \<midarrow>a\<midarrow>the_ioa\<longrightarrow> t" and "safe_at s i v b"
+  shows "safe_at t i v b" using assms ballot_array_prefix.safe_at_mono
+by (metis ballot_array_prefix_axioms.intro ballot_array_prefix_def quorums_axioms trans_imp_prefix_order)
+
+abbreviation safe where "safe s \<equiv> \<forall> i . ballot_array.safe  quorums (ballot s) (vote s i)"
+  
+lemma safe_votes:
+  assumes "s \<midarrow>aa\<midarrow>the_ioa\<longrightarrow> t" and "vote s i a b  \<noteq> vote t i a b" and "vote t i a b = Some v"
+    and "conservative_array s" and "safe s"
+  shows "safe_at t i v b" 
+  using assms
+  apply (cases aa)
+    apply (auto simp add:inv_proofs_defs)
+  subgoal premises prems
+  proof -
+    have "safe_at s i v (ballot s a)" by (smt assms(4) ballot_array.safe_def ballot_array_props.intro ballot_array_props.proved_safe_at_abs_imp_safe_at option.case_eq_if option.distinct(1) option.sel prems(2) prems(6) quorums_axioms) 
+    thus ?thesis by (metis amp_state.select_convs(2) amp_state.select_convs(3) amp_state.surjective amp_state.update_convs(3) assms(1) fun_upd_apply prems(9) safe_mono) 
+  qed
+  done
+
+lemma safe_inv:
+  "invariant the_ioa safe"
+apply (try_solve_inv2 case_thm:trans_cases inv_proofs_defs:inv_proofs_defs ballot_array.safe_def invs:invs)
+subgoal premises prems for s t act
+proof (auto simp add:ballot_array.safe_def split:option.splits)
+  fix i b a v
+  assume "vote t i a b = Some v"
+  show "safe_at t i v b"
+  proof (cases "vote s i a b = vote t i a b")
+    case True
+    hence "safe_at s i v b" using prems(1) by (metis \<open>vote t i a b = Some v\<close> ballot_array.safe_def option.simps(5))
+    thus ?thesis using prems(2) safe_mono
+      by fastforce 
+  next
+    case False thus ?thesis using safe_votes
+      using \<open>vote t i a b = Some v\<close> prems(1-3) by blast  
+  qed
+qed
+done
+declare safe_inv[invs]
+
+subsection {* Finally, the proof that agreement holds (trivial, follows immediately from safe).*}
+
+definition agreement where 
+  "agreement s \<equiv> \<forall> v w i . chosen s i v \<and> chosen s i w \<longrightarrow> v = w"
+
+lemma agreement:"invariant the_ioa agreement"
+apply(rule invariantI)
+    apply(auto simp add: inv_proofs_defs agreement_def ballot_array.chosen_def ballot_array.chosen_at_def)[1]
+  apply (metis (mono_tags, lifting) IOA.invariant_def IOA.reachable_n agreement_def amp_proof.safe_inv amp_proof_axioms ballot_array_props.intro ballot_array_props.safe_imp_agreement quorums_axioms the_ioa_def)
+done
+
+end
+
+end
