Isabelle2/DistributedSafeAt_code.thy
@@ -1,0 +1,15 @@
+section {* Just checking that code generation works *}
+
+theory DistributedSafeAt_code
+  imports DistributedSafeAt
+begin
+
+global_interpretation dsa:distributed_safe_at quorums ballot vote for quorums ballot vote 
+  defines acc_max = dsa.acc_max and max_quorum_votes = dsa.max_quorum_votes .
+
+term acc_max
+thm acc_max_def
+
+export_code acc_max in Scala
+
+end
