Isabelle2/R3_Refines_R1.thy
@@ -1,0 +1,709 @@
+section {* R3 refines R1 *} 
+
+theory R3_Refines_R1   
+imports AbstractMultiPaxosR3 AbstractMultiPaxosR1 Simulations Hist_Supplemental IOA_Automation
+begin
+
+section {* A few lemmas *}
+
+lemma comprehension_to_fold:
+  fixes Y P c
+  assumes "finite Y" 
+  defines "c \<equiv> \<lambda> y xs . xs \<union> {x . P x y}"
+  shows "{x . \<exists> y \<in> Y . P x y} = Finite_Set.fold c {} Y" using assms
+proof -
+  interpret c_folding:folding_idem c "{}"
+    apply (unfold_locales)
+     apply (auto simp add:c_def)
+    done
+  show ?thesis using assms(1)
+  proof (induct Y)
+    case empty
+    then show ?case by simp
+  next
+    case (insert x F)
+    have "Finite_Set.fold c {} (insert x F) = c x {x . \<exists> y \<in> F . P x y}"
+      using c_folding.eq_fold c_folding.insert insert.hyps(1) insert.hyps(2) insert.hyps(3) by auto
+    also have "... =  {z . \<exists> y \<in> (insert x F) . P z y}" 
+      by (fastforce simp add:c_def)
+    finally show ?case by simp
+  qed
+qed
+
+lemma comprehension_to_fold_2:
+  fixes f S P g i c
+  assumes "finite S"
+  defines "c \<equiv> \<lambda> a res . (\<lambda> (gai, ri) . if P gai then insert (f gai) ri else ri) o$ ($ g a, res $)"
+  shows
+    "{f ((g a) $ i) | a . a \<in> S \<and> P ((g a) $ i)} = (Finite_Set.fold c (K$ {}) S) $ i" using assms(1)
+proof (induct)
+  case empty
+  then show ?case by simp
+next
+  case (insert x F)
+  interpret c_folding:folding_idem c "K$ {}"
+    apply (unfold_locales)
+     apply (auto simp add:c_def fun_eq_iff expand_finfun_eq)
+    done
+  have 1:"\<And> ff . c x ff $ i = (if P (g x $ i) then insert (f (g x $ i)) (ff $ i) else ff $ i)"
+    by (simp add:c_def)
+  have "Finite_Set.fold c (K$ {}) (insert x F) $ i = c x (Finite_Set.fold c (K$ {}) F) $ i"
+    using c_folding.eq_fold c_folding.insert_idem insert.hyps(1) by auto
+  also have "... = (if (P (g x $ i)) then insert (f (g x $ i)) (Finite_Set.fold c (K$ {}) F $ i)
+    else (Finite_Set.fold c (K$ {}) F) $ i)"
+    by (simp add: "1")
+  finally show ?case using insert.hyps
+    by auto
+qed
+
+locale receive_1b_lemmas = receive_1b onebs as log for onebs as log +
+  assumes votes_default:"\<And> a . finfun_default (onebs $ a) = None"
+    and log_default:"finfun_default log = inst_status.Free" and fin:"finite as"
+  and conservative:"\<And> a a' i b v v' . \<lbrakk>onebs $ a $ i = Some (v,b); onebs $a' $ i = Some (v',b)\<rbrakk>
+        \<Longrightarrow> v = v'"
+begin
+
+lemma votes_per_inst_decl:
+  "votes_per_inst $ i = {the (onebs $ a $ i) | a . a \<in> as \<and> onebs $ a $ i \<noteq> None}"
+proof -
+  let ?f="\<lambda>(gai, ri). if gai \<noteq> None then insert (the gai) ri else ri"
+  have 1:"?f = (\<lambda> (vo, vs) . option_as_set vo \<union> vs)"
+    by (auto simp add:option_as_set_def fun_eq_iff split!:option.splits)
+  have 2:"votes_per_inst = Finite_Set.fold (\<lambda> a vs . ?f o$ ($ (onebs $ a), vs $)) (K$ {}) as"
+    by (simp only:votes_per_inst_def 1 Let_def pre_votes_per_inst_def c_def[abs_def])
+  note 3 = comprehension_to_fold_2[OF fin, where ?g="op$ onebs" and ?f=the and ?P="flip op\<noteq> None"]
+  show ?thesis by (simp only:2 3)
+qed
+  
+lemma votes_per_inst_default:
+  assumes "\<And> a . finfun_default (onebs $ a) = None"
+  shows "finfun_default votes_per_inst = {}" using fin
+proof (simp add:votes_per_inst_def, induct)
+  case empty
+  then show ?case by (simp add:pre_votes_per_inst_def)
+next
+  case (insert x F)
+    have 1:"Finite_Set.fold c (K$ {}) (insert x F) = c x (Finite_Set.fold c (K$ {}) F)" using insert_idem
+      by (simp add: eq_fold insert.hyps(1))
+    have "finfun_default (Finite_Set.fold c (K$ {}) F) = {}" using insert.hyps(3) insert.prems
+      by (simp add: pre_votes_per_inst_def)
+    moreover have "finfun_default (onebs $ x) = None"
+      by (simp add: assms)  
+    ultimately have "finfun_default ($ onebs $ x, Finite_Set.fold c (K$ {}) F $) = (None, {})"
+      by (simp add: diag_default)
+    with 1 show ?case by (simp add:c_def pre_votes_per_inst_def comp_default option_as_set_def)
+qed
+
+lemma max_per_inst_default:
+  "finfun_default (max_per_inst) = {}"
+proof -
+  have "finfun_default votes_per_inst = {}"
+    using votes_default votes_per_inst_default by auto
+  thus ?thesis by (simp add:max_per_inst_def max_by_key_def comp_default)
+qed
+
+lemma new_log_default:
+  "finfun_default new_log = inst_status.Free" using log_default
+  by (auto simp add:new_log_def max_per_inst_default comp_default diag_default)
+
+lemma conservative_per_inst:
+  fixes v v' b i
+    assumes "(v,b) \<in> votes_per_inst $ i"
+    and "(v',b) \<in> votes_per_inst $ i"
+  shows "v = v'" using conservative assms votes_per_inst_decl
+proof -
+  have "(v, b) \<in> {the (onebs $ a $ i) |a. a \<in> as \<and> onebs $ a $ i \<noteq> None}"
+    by (metis assms(1) votes_per_inst_decl)
+  then have f1: "\<exists>a. (v, b) = the (onebs $ a $ i) \<and> a \<in> as \<and> onebs $ a $ i \<noteq> None"
+  proof -
+    show ?thesis
+      using \<open>(v, b) \<in> {the (onebs $ a $ i) |a. a \<in> as \<and> onebs $ a $ i \<noteq> None}\<close> by auto
+  qed
+  have "(v', b) \<in> {the (onebs $ a $ i) |a. a \<in> as \<and> onebs $ a $ i \<noteq> None}"
+    by (metis assms(2) votes_per_inst_decl)
+  then have "\<exists>a. (v', b) = the (onebs $ a $ i) \<and> a \<in> as \<and> onebs $ a $ i \<noteq> None"
+  proof -
+    show ?thesis
+      using \<open>(v', b) \<in> {the (onebs $ a $ i) |a. a \<in> as \<and> onebs $ a $ i \<noteq> None}\<close> by auto
+  qed
+  then show ?thesis
+    using f1 by (metis conservative option.collapse)
+qed
+
+lemma max_per_inst_lemma:
+  "\<forall> i . max_per_inst $ i = max_by_key {(v,b) . (\<exists> a \<in> as . onebs $ a $ i = Some (v,b))} snd"
+  apply (rule allI) 
+  apply (simp add:votes_per_inst_decl max_per_inst_def)
+  by (smt Collect_cong case_prodE case_prodI option.sel)
+  
+lemma new_log_lemma:
+  "\<forall> i . let m = max_by_key {(v,b) . (\<exists> a \<in> as . onebs $ a $ i = Some (v,b))} snd in
+     case log $ i of Decided _ \<Rightarrow> new_log $ i = log $ i
+     | _ \<Rightarrow> if m = {} then new_log $ i = Free
+        else new_log $ i = Active"
+  apply (rule allI) apply (auto simp add:Let_def new_log_def split!:inst_status.splits)
+     apply (metis empty_iff max_per_inst_lemma)
+    apply (metis empty_iff max_per_inst_lemma)
+   apply (metis empty_iff max_per_inst_lemma)
+  by (metis empty_iff max_per_inst_lemma)
+
+lemma msgs_lemma:
+  "msgs = {Phase2a i b v | i b v . (new_log $ i = Active \<and> max_per_inst $ i = {(v,b)})}"
+proof -
+  have 1:"finfun_default ((op= Active) o$ new_log) = False" using new_log_default
+    apply auto
+  proof -
+    assume a1: "finfun_default (op = Active \<circ>$ local.new_log)"
+    assume a2: "finfun_default local.new_log = Free"
+    have "Active = finfun_default local.new_log"
+      using a1 comp_default by auto
+    then show False
+      using a2 by (metis inst_status.distinct(5))
+  qed
+  hence "i \<in> set (finfun_to_list ((op= Active) o$ new_log)) = (new_log $ i = Active)" for i
+    apply (simp add:)
+  proof -
+    assume a1: "\<not> finfun_default (op = Active \<circ>$ local.new_log)"
+    have f2: "\<And>p f n i. (p \<circ>$ f(n::nat $:= i::'b inst_status)) $ n \<or> \<not> p i"
+      by (metis finfun_comp_update finfun_upd_apply)
+    have f3: "\<And>f n i. f(n::nat $:= i::'b inst_status) = f \<or> i \<noteq> f $ n"
+      by (metis finfun_ext finfun_upd_apply)
+    then have f4: "\<And>p f n. p (f $ (n::nat)::'b inst_status) \<or> \<not> (p \<circ>$ f) $ n"
+      by (metis finfun_comp_update finfun_upd_apply)
+    { assume "Active \<noteq> local.new_log $ i \<and> local.new_log $ i \<noteq> Active"
+      then have "\<not> (op = Active \<circ>$ local.new_log) $ i \<and> \<not> finfun_default (op = Active \<circ>$ local.new_log) \<and> local.new_log $ i \<noteq> Active"
+        using f4 a1 by metis
+      then have "finfun_dom (op = Active \<circ>$ local.new_log) $ i = (local.new_log $ i = Active)"
+        by (smt finfun_dom_conv) }
+    then show "finfun_dom (op = Active \<circ>$ local.new_log) $ i = (local.new_log $ i = Active)"
+      using f3 f2 a1 by (metis finfun_dom_conv)
+  qed 
+  thus ?thesis unfolding msgs_def Let_def apply simp 
+    (* Here we are missing the fact that if an instance is Active in new_log then its max_per_inst
+    is a singleton*)
+  oops
+  
+end
+  
+section {* Refinement proof using a refinement mapping *}
+  
+locale ref_proof_4 = quorums quorums + amp_r3 leader next_bal as quorums
+  + r1:ampr1_ioa quorums leader
+  for quorums :: "('a::linorder) set set" and leader :: "bal \<Rightarrow> ('a::linorder)" and next_bal as + 
+  fixes ampr3_ioa :: "(('a, 'v) global_state, 'v paxos_action) ioa" 
+    and ampr1_ioa :: "(('v, 'a, 'l) ampr1_state, 'v paxos_action) ioa" 
+  defines "ampr3_ioa \<equiv> ioa" and "ampr1_ioa \<equiv> r1.ioa"
+  fixes a1 a2 a3
+  assumes at_least_3:"a1 \<in> as \<and> a2 \<in> as \<and> a3 \<in> as \<and> a1 \<noteq> a2 \<and> a3 \<noteq> a2 \<and> a3 \<noteq> a1"
+  assumes fin:"finite as" and infin:"infinite (UNIV::'a set)"
+    -- {* @{term "UNIV::'a set"} must be infinite for @{term finfun_default} to make sense. *}
+begin
+
+interpretation IOA .
+
+lemmas action_defs = propose_def do_2a_def receive_2b_def
+      try_acquire_leadership_def receive_1a_def receive_2a_def receive_1b_def receive_fwd_def
+  send_all_def Let_def
+
+lemmas init_defs = ampr3_ioa_def ioa_def global_start_def local_start_def
+  ampr1_ioa_def r1.ioa_def r1.start_def r1.start_s_def 
+
+method trans_cases =
+  (simp add:is_trans_def ampr3_ioa_def ioa_def, elim trans_cases)
+
+definition inv1 where inv1_def[inv_proofs_defs]:
+  "inv1 s \<equiv> \<forall> a . acceptors (lstate s a) = as \<and> id (lstate s a) = a"
+lemma inv1:"invariant ampr3_ioa inv1"
+  apply (rule invariantI)
+   apply (simp add:inv1_def init_defs)
+  apply (rm_reachable)
+  apply trans_cases
+         apply (auto simp add:inv1_def action_defs)
+  done
+declare inv1[invs]
+
+declare finfun_upd_apply[simp]
+
+definition inv6 where inv6_def:
+  "inv6 s \<equiv> \<forall> a i b v . (Packet a (Phase2a i b v) \<in> network s \<longrightarrow> log (lstate s (leader b)) $ i \<noteq> Free)"
+lemma inv6: "invariant ampr3_ioa inv6"
+  apply (rule invariantI)
+   apply (simp add:inv6_def init_defs)
+  apply (insert invs)
+  apply (instantiate_invs)
+  apply (rm_reachable)
+  apply (trans_cases)
+        apply (fastforce simp add:inv1_def inv6_def action_defs)
+        apply (fastforce simp add:inv1_def inv6_def action_defs)
+       apply (simp add:inv1_def inv6_def action_defs split!:if_splits)
+      apply (fastforce simp add:inv1_def inv6_def action_defs split!:if_splits)
+     apply (fastforce simp add:inv1_def inv6_def action_defs split!:if_splits)
+    apply (fastforce simp add:inv1_def inv6_def action_defs split!:if_splits) defer
+   apply (fastforce simp add:inv1_def inv6_def action_defs split!:if_splits)
+   (* TODO: The hard one is left. *) oops
+  
+definition inv2 where inv2_def:
+  "inv2 s \<equiv> \<forall> i b v1 v2 a1 a2 .
+    (Packet a1 (Phase2a i b v1) \<in> network s
+      \<and> Packet a2 (Phase2a i b v2) \<in> network s \<longrightarrow> v1 = v2)"
+lemma inv2:"invariant ampr3_ioa inv2"
+  apply (rule invariantI)
+   apply (simp add:inv2_def init_defs)
+  apply (insert invs)
+  apply (instantiate_invs)
+  apply (rm_reachable)
+  apply (trans_cases;
+    (simp add:inv1_def inv2_def action_defs finfun_default_update_const split!:packet.splits msg.splits; fail)?)
+  subgoal premises prems for s t act a v
+  proof -
+    thm prems
+    show ?thesis using prems(1,2,4) oops
+      nitpick[no_assms, card 'v =2, card 'a = 1, show_types]
+  
+definition inv3 where 
+  "inv3 s \<equiv> \<forall> i a1 a2 b d1 v1 d2 v2 .
+    Packet d1 (Phase2b a1 i b v1) \<in> network s \<and> Packet d2 (Phase2b a2 i b v2) \<in> network s
+    \<longrightarrow> v1 = v2"
+lemma inv2:"invariant ampr3_ioa inv2"
+  apply (rule invariantI)
+   apply (simp add:inv2_def init_defs)
+  apply (insert invs)
+  apply (instantiate_invs)
+  apply (rm_reachable)
+  apply trans_cases
+  oops
+
+definition inv5 :: "('a,'v)global_state \<Rightarrow> bool" where inv5_def[inv_proofs_defs]:
+  "inv5 s \<equiv> \<forall> a b a2 p . 
+    finfun_default ((acc.onebs (lstate s a)) $ b $ a2) = None
+    \<and> (finfun_default (acc.votes (lstate s a)) = None)
+    \<and> (p \<in> network s \<longrightarrow> 
+        (case p of Packet _ (Phase1b _ _ vs) \<Rightarrow> finfun_default vs = None
+        | Packet _ _ \<Rightarrow> True))"
+lemma inv5:"invariant ampr3_ioa inv5"
+  apply (rule invariantI)
+   apply (simp add:inv5_def init_defs finfun_default_const)
+  apply (insert invs)
+  apply (instantiate_invs)
+  apply (rm_reachable)
+  apply (trans_cases;
+    (simp add:inv1_def inv5_def action_defs finfun_default_update_const split!:packet.splits msg.splits; fail)?)
+  subgoal premises prems for s t act a b vs m p a2 (* receive_1b*)
+  proof -
+    have 1:"acc.onebs (lstate t a) = new_onebs (acc.onebs (lstate s a)) vs b a2"
+      using prems(2,5,6) by (auto simp add:inv1_def action_defs)
+    show ?thesis
+    proof (auto simp add:inv5_def)
+      fix a' b' a2'
+      show "finfun_default (acc.onebs (lstate t a') $ b' $ a2') = None" 
+      proof (cases "a' = a")
+        case True
+        have 2:"acc.onebs (lstate t a') = new_onebs (acc.onebs (lstate s a')) vs b a2"
+          using 1 True by auto
+        have 3:"finfun_default (acc.onebs (lstate s a') $ b' $ a2') = None"
+          using prems(1) by (auto simp add:inv5_def)
+        show ?thesis using 2 3 prems(1,4,7)
+          apply (auto simp add: inv5_def new_onebs_def update_onebs.new_onebs_def)
+          apply (case_tac "b' = b", case_tac "a2' = a2")
+            apply fastforce
+          apply blast
+          by fastforce
+      next
+        case False
+        then show ?thesis using prems(1,6) by (simp add:inv5_def) 
+      qed
+    next
+      fix a
+      show "finfun_default (votes (lstate t a)) = None" using prems 
+        by (simp add:inv1_def inv5_def action_defs finfun_default_update_const split!:packet.splits msg.splits)
+    next 
+      fix p
+      let ?sa = "lstate s a"
+      have 1:"let msgs = msgs (acc.onebs ?sa $ b) (acc.acceptors ?sa) (log ?sa)
+        in snd (receive_1b ?sa a2 b vs) \<subseteq> \<Union> {send_all ?sa m | m . m \<in> msgs} "
+        by (auto simp add:inv1_def action_defs)
+      have 2:"\<And> m . let msgs = msgs (acc.onebs ?sa $ b) (acc.acceptors ?sa) (log ?sa) in 
+        m \<in> \<Union> {send_all ?sa m | m . m \<in> msgs} \<Longrightarrow> case m of Packet _ (Phase2a _ _ _) \<Rightarrow> True | _ \<Rightarrow> False"
+        using r1.msgs_lemma by (fastforce simp add:send_all_def)
+      from 1 2 have "\<And> p . p \<in> snd (receive_1b ?sa a2 b vs) \<Longrightarrow> 
+        case p of Packet _ (Phase2a _ _ _) \<Rightarrow> True | _ \<Rightarrow> False" by auto
+      moreover have "network t = snd (receive_1b ?sa a2 b vs) \<union> network s" using prems(5,6) by auto
+      ultimately show "p \<in> network t \<Longrightarrow> case p of Packet _ (Phase1b _ _ vs) \<Rightarrow> finfun_default vs = None | Packet _ _ \<Rightarrow> True"  
+        using prems(1) by (force simp add:inv5_def inv1_def split!:packet.splits msg.splits)
+    qed
+  qed
+  done
+declare inv5[invs]
+
+definition inv4 where "inv4 s \<equiv>
+  (\<forall> a . finfun_default (log (lstate s a)) = Free)"
+  
+lemma inv4:"invariant ampr3_ioa inv4"
+  apply (rule invariantI)
+   apply (simp add:inv4_def init_defs)
+   apply (simp add: finfun_default_const)
+  apply (insert invs)
+  apply (instantiate_invs)
+  apply (rm_reachable)
+  apply trans_cases
+         apply (auto simp add:inv4_def inv1_def action_defs finfun_default_update_const finfun_upd_apply
+          amp_r3.next_inst_lemma
+          split!:if_splits msg.splits packet.splits inst_status.splits) oops
+
+fun extract_vs where 
+  "extract_vs (Fwd v) = {v}"
+| "extract_vs (Phase2a _ _ v) = {v}"
+| "extract_vs (Phase2b _ _ _ v) = {v}"
+| "extract_vs (Phase1b _ _ ff) = {v . \<exists> i b . ff $ i = Some (v,b)}"
+  -- {* Could be @{term "{ff $ i \<bind> (Some o fst) | i . True} \<bind> option_as_set" } *}
+| "extract_vs _ = {}"
+  
+definition propCmd where "propCmd s \<equiv> \<Union> ((\<lambda> p . case p of Packet _ m \<Rightarrow> extract_vs m) ` network s)"
+
+definition ref_map where "ref_map s \<equiv> \<lparr>
+  ampr1_state.propCmd = propCmd s,
+  ballot = \<lambda> a . acc.ballot (lstate s a),
+  vote = \<lambda> i a b . if (\<exists> a2 v . Packet a2 (Phase2b a i b v) \<in> network s) 
+    then Some (the_elem {v . \<exists> a2 . Packet a2 (Phase2b a i b v) \<in> network s}) else None,
+  suggestion = \<lambda> i b . if (\<exists> a v. Packet a (Phase2a i b v) \<in> network s) 
+    then Some (the_elem {v . \<exists> a . Packet a (Phase2a i b v) \<in> network s}) else None,
+  onebs = \<lambda> a b . if (\<exists> ff . Packet (leader b) (Phase1b a b ff) \<in> network s) 
+    then Some (the_elem {op$ ff | ff . Packet (leader b) (Phase1b a b ff) \<in> network s}) else None\<rparr>"
+  
+lemmas ref_defs = ref_map_def propCmd_def 
+
+lemma "is_ref_map ref_map ampr3_ioa ampr1_ioa"
+  apply (auto simp add:is_ref_map_def)
+   apply (simp add:init_defs ref_defs)
+  apply (insert invs)
+  apply (instantiate_invs)
+  apply (rm_reachable)
+  apply trans_cases
+  subgoal premises prems for s t act a v (* Propose *)
+  proof (intro exI[where ?x="ref_map s"] exI[where ?x="[(act, ref_map t)]"])
+    thm prems
+    have "ref_map t = (ref_map s)\<lparr>propCmd := insert v (ampr1_state.propCmd (ref_map s))\<rparr>"
+    proof (cases "leader (acc.ballot (lstate s a)) = a") oops
+    
+end
+
+section {* Testing interpretation. *}
+
+
+definition n :: nat where "n \<equiv> 3"
+  -- {* The number of processes *}
+
+definition accs where "accs \<equiv> {1..n}"
+  -- {* The set of acceptors *}
+
+definition leader where "leader (b::nat) \<equiv> (b mod n) + 1"
+  
+definition next_bal :: "nat \<Rightarrow> nat \<Rightarrow> nat" where "next_bal b a \<equiv> 
+  (b div n + 1) * n + a"
+
+global_interpretation cq:card_quorums accs
+  defines qs = "cq.quorums" and nas = "cq.nas"
+  apply (unfold_locales)
+   apply (simp add: accs_def n_def)
+  apply (simp add: accs_def)
+  done
+                
+definition r3_ioa :: "((nat, nat) global_state, nat paxos_action) ioa"
+  where r3_ioa_def:"r3_ioa \<equiv> amp_r3.ioa leader next_bal accs"
+
+definition r1_ioa  :: "((nat, nat, nat) ampr1_state, nat paxos_action) ioa"
+  where "r1_ioa \<equiv> ampr1_ioa.ioa qs leader"
+  
+global_interpretation ref_proof_4 qs leader next_bal accs 
+  r3_ioa r1_ioa 1 2 3
+    apply (unfold_locales)
+      apply (auto simp add:accs_def n_def r3_ioa_def r1_ioa_def) .
+
+term ioa
+thm ioa_def
+interpretation IOA .
+thm init_defs
+(* declare [[show_types, show_consts]] *)
+lemma "invariant r3_ioa inv2"
+  apply (rule invariantI)
+   apply (simp add:inv2_def init_defs accs_def leader_def next_bal_def amp_r3.ioa_def
+      amp_r3.global_start_def)
+  apply (insert invs)
+  apply (instantiate_invs)
+  apply (rm_reachable)
+  apply (trans_cases;
+    (simp add:inv1_def inv2_def action_defs finfun_default_update_const split!:packet.splits msg.splits; fail)?)
+apply (simp add:inv2_def inv1_def inv5_def propose_def do_2a_def send_all_def) oops
+  
+section {* Old attempts. *}
+
+subsection {* Proof using a history variable (simple sketch) *}
+
+locale ref_proof_1 = quorums quorums + amp_r3 leader next_bal as quorums 
+  + r1:ampr1_ioa quorums leader
+  for quorums :: "('a::linorder) set set" and leader :: "bal \<Rightarrow> ('a::linorder)" and next_bal as + 
+  fixes ampr3_ioa :: "(('a, 'v) global_state, 'v paxos_action) ioa" 
+    and ampr1_ioa :: "(('v, 'a, 'l) ampr1_state, 'v paxos_action) ioa" 
+  defines "ampr3_ioa \<equiv> ioa" and "ampr1_ioa \<equiv> r1.ioa"
+begin
+
+interpretation IOA .
+
+definition ghost_ioa where 
+  -- {* We add a history variable that tracks the set of proposed commands. *}
+  "ghost_ioa \<equiv>
+      let update = \<lambda> s h a s' . case a of Propose v \<Rightarrow> insert v h | _ \<Rightarrow> h;
+        init = \<lambda> s . {}
+      in
+    add_history ampr3_ioa update init"
+
+lemmas ioa_defs =
+   IOA.actions_def
+   IOA.externals_def IOA.add_history_def
+
+lemmas amp_defs = ioa_defs ampr1_ioa_def ampr3_ioa_def ghost_ioa_def
+  ioa_def global_start_def
+
+definition inv1 where "inv1 s \<equiv> let r3_s = fst s; h = snd s in
+  \<forall> a v . (Packet a (Fwd v)) \<in> network r3_s \<longrightarrow> v \<in> h"
+declare inv1_def[inv_proofs_defs]
+
+lemma inv1:"invariant ghost_ioa inv1"
+  apply (rule invariantI)
+   apply (simp add:inv1_def amp_defs)
+  apply (rm_reachable)
+  apply (simp add:ghost_ioa_def)
+  apply (simp only: split_paired_all)
+  apply (frule IOA.add_hist_trans(1), drule IOA.add_hist_trans(2))
+  apply (simp add:is_trans_def ampr3_ioa_def ioa_def)
+  apply (drule trans_cases)
+          apply (auto simp add:inv1_def)
+         defer 
+         apply(simp add:receive_2b_def Let_def split:if_splits option.splits)
+        apply(simp add:try_acquire_leadership_def Let_def send_all_def split:if_splits option.splits)
+       apply (metis amp_r3.msg.distinct(13) amp_r3.packet.inject empty_iff receive_1a_def singletonD snd_conv)
+      apply(simp add:receive_2a_def Let_def send_all_def split:if_splits option.splits)
+     apply(simp add:receive_2b_def Let_def send_all_def split:if_splits option.splits)
+    apply(simp add:receive_1b_def receive_1b.msgs_def msgs_def Let_def send_all_def split:if_splits option.splits)
+  subgoal proof - oops
+    fix a :: "('a, 'v) global_state" and b :: "'v set" and ac :: 'a and bb :: nat and vs :: "nat \<Rightarrow>f ('v \<times> nat) option" and ad :: "('a, 'v) acc" and bc :: "('a, 'v) packet set" and ae :: 'a and v :: 'v
+    assume a1: "(\<exists>x. finfun_dom (receive_1b.new_log (the (acc.onebs (lstate a ac) $ bb)) (acceptors (lstate a ac)) (log (lstate a ac))) $ x \<and> (Fwd v::('a, 'v) msg) = (case the_elem (receive_1b.max_per_inst (the (acc.onebs (lstate a ac) $ bb)) (acceptors (lstate a ac)) $ x) of (v, b) \<Rightarrow> Phase2a x b v)) \<and> ae \<in> acceptors (lstate a ac) \<and> ae \<noteq> acc.id (lstate a ac)"
+    have "\<And>n p v. (case p of (v, na) \<Rightarrow> Phase2a n na v) \<noteq> (Fwd v::('a, 'v) msg)"
+      by (metis amp_r3.msg.distinct(17) case_prod_conv surj_pair)
+    then show "v \<in> b"
+      using a1 by metis
+  qed
+   apply(simp add: do_2a_def receive_fwd_def Let_def send_all_def split:if_splits option.splits)
+  apply(simp add: do_2a_def propose_def Let_def send_all_def split:if_splits option.splits)
+  done
+
+end
+
+subsection {* Proof using a more involved history state. *}
+  
+locale ref_proof = quorums quorums + amp_r3 leader next_bal as quorums 
+  + r1:ampr1_ioa quorums leader
+  for quorums :: "('a::linorder) set set" and leader :: "bal \<Rightarrow> ('a::linorder)" and next_bal as + 
+  fixes ampr3_ioa :: "(('a, 'v) global_state, 'v paxos_action) ioa" 
+    and ampr1_ioa :: "(('v, 'a, 'l) ampr1_state, 'v paxos_action) ioa" 
+  defines "ampr3_ioa \<equiv> ioa" and "ampr1_ioa \<equiv> r1.ioa"
+begin
+
+interpretation IOA .
+
+lemmas ioa_defs =
+   IOA.actions_def
+   IOA.externals_def IOA.add_history_def
+
+definition update_hist where "update_hist s h a s' \<equiv> case a of 
+  Propose v \<Rightarrow> h\<lparr>propCmd := insert v (propCmd h)\<rparr>
+  | Internal \<Rightarrow> 
+      h\<lparr>vote := \<lambda> i a b . case (votes (lstate s' a) $ i) of Some (v,b2) \<Rightarrow> 
+          (if b = b2 then Some v else (vote h i a b)) | None \<Rightarrow> None,
+        ampr1_state.ballot := \<lambda> a . acc.ballot (lstate s' a),
+        suggestion := \<lambda> i b . case (log (lstate s' (leader b)) $ i) of Proposed v \<Rightarrow> (
+              case (log (lstate s (leader b)) $ i) of Free \<Rightarrow> Some v | _ \<Rightarrow> suggestion h i b)
+          | Decided v \<Rightarrow> suggestion h i b
+          | Free \<Rightarrow> None,
+        onebs := \<lambda> a b . if acc.ballot (lstate s' a) = b \<and> acc.ballot (lstate s' a) \<noteq> b
+          then Some (op$ (votes (lstate s a))) else None\<rparr>
+  | _ \<Rightarrow> h"
+
+definition ghost_ioa where 
+  -- {* This gets a little tricky. Why not define a history IOA without @{term add_hist} and 
+  prove trace inclusion with a forward simulation? *}
+  "ghost_ioa \<equiv> add_history ampr3_ioa update_hist (\<lambda> s . r1.start_s)"
+
+lemmas amp_defs = ioa_defs ampr1_ioa_def ampr3_ioa_def ghost_ioa_def
+  ioa_def global_start_def
+
+definition inv1 where "inv1 s \<equiv> let r3_s = fst s; h = snd s in
+  \<forall> a v . (Packet a (Fwd v)) \<in> network r3_s \<longrightarrow> v \<in> propCmd h"
+declare inv1_def[inv_proofs_defs]
+
+lemma inv1:"invariant ghost_ioa inv1"
+  apply (rule invariantI)
+   apply (simp add:inv1_def amp_defs)
+  apply (rm_reachable)
+  apply (simp add:ghost_ioa_def)
+  apply (simp only: split_paired_all)
+  apply (frule IOA.add_hist_trans(1), drule IOA.add_hist_trans(2))
+  apply (simp add:is_trans_def ampr3_ioa_def ioa_def)
+  apply (elim trans_cases)
+         apply (auto simp add:inv1_def update_hist_def)
+         apply (simp add:propose_def do_2a_def Let_def send_all_def split:if_splits)
+        apply (simp add:receive_2b_def Let_def send_all_def split:if_splits)
+       apply (simp add:try_acquire_leadership_def Let_def send_all_def split:if_splits)
+      apply (simp add:receive_1a_def Let_def send_all_def split:if_splits)
+     apply (simp add:receive_2a_def Let_def send_all_def split:if_splits)
+    apply (simp add:receive_2b_def Let_def send_all_def split:if_splits)
+   apply (simp add:receive_1b_def Let_def send_all_def msgs_def receive_1b.msgs_def split:if_splits)
+  subgoal proof -
+    fix a :: "('a, 'v) global_state" and b :: "('v, 'a, ?'l) ampr1_state" and ac :: 'a and bb :: nat and vs :: "nat \<Rightarrow>f ('v \<times> nat) option" and ad :: "('a, 'v) acc" and bc :: "('a, 'v) packet set" and ae :: 'a and v :: 'v
+    assume a1: "(\<exists>x. finfun_dom (receive_1b.new_log (the (acc.onebs (lstate a ac) $ bb)) (acceptors (lstate a ac)) (log (lstate a ac))) $ x \<and> (Fwd v::('a, 'v) msg) = (case the_elem (receive_1b.max_per_inst (the (acc.onebs (lstate a ac) $ bb)) (acceptors (lstate a ac)) $ x) of (v, b) \<Rightarrow> Phase2a x b v)) \<and> ae \<in> acceptors (lstate a ac) \<and> ae \<noteq> acc.id (lstate a ac)"
+    have "\<And>n p v. (case p of (v, na) \<Rightarrow> Phase2a n na v) \<noteq> (Fwd v::('a, 'v) msg)"
+      by (metis amp_r3.msg.distinct(17) case_prod_conv surj_pair)
+    then show "v \<in> propCmd b" oops
+      using a1 by metis
+  qed
+  apply (simp add:receive_fwd_def do_2a_def Let_def send_all_def split:if_splits)
+  done
+declare inv1[invs]
+
+definition ref_map where "ref_map s \<equiv> snd s"
+  
+method apply_exI_hist =
+  (match conclusion in "\<exists> e\<^sub>0 ef . refines (e\<^sub>0,ef) (?s,h) a (?s',h') ?ioa ?f" for h h' a 
+    \<Rightarrow> \<open>intro exI[where ?x=h] exI[where ?x="[(a,h')]"]\<close>)
+
+lemma "is_ref_map ref_map ghost_ioa ampr1_ioa"
+  apply (auto simp add:is_ref_map_def)
+   apply (simp add:ghost_ioa_def add_history_def ampr3_ioa_def r1.start_s_def ampr1_ioa_def r1.ioa_def r1.start_def
+      ref_map_def)
+  apply (insert invs)
+  apply (instantiate_invs)
+  apply (rm_reachable)
+  apply (simp add:ghost_ioa_def)
+  apply (frule IOA.add_hist_trans(1), drule IOA.add_hist_trans(2))
+  apply (simp add:is_trans_def ampr3_ioa_def ioa_def)
+  apply (elim trans_cases)
+  (* Propose. *)
+         apply apply_exI_hist
+         apply (force simp add:ampr1_ioa_def ref_map_def refines_def update_hist_def is_trans_def r1.ioa_def
+      r1.trans_def trace_match_def paxos_asig_def Let_def inv1_def r1.propose_def externals_def
+      trace_def schedule_def filter_act_def propose_def do_2a_def split!:if_splits)
+        prefer 7
+  subgoal premises prems for s h s' h' act a v m p
+    apply apply_exI_hist
+    apply (simp add:refines_def)
+    apply (intro conjI)
+       apply (simp add:ref_map_def)
+      apply (simp add:ref_map_def)
+     prefer 2
+     apply (simp add:trace_match_def trace_def schedule_def externals_def
+        filter_act_def ampr1_ioa_def r1.ioa_def paxos_asig_def Let_def split!:if_splits)
+  subgoal proof (cases "id (lstate s a) = leader (acc.ballot (lstate s a))")
+    case False
+    with prems(3,5,6) have "update_hist s h act s' = h" apply (simp add:update_hist_def receive_fwd_def)
+    thm prems
+    oops
+    
+end
+
+subsection {* implementation proof using a forward simulation *}
+  
+locale ref_proof_3 = quorums quorums + amp_r3 leader next_bal as quorums
+  + r1:ampr1_ioa quorums leader
+  for quorums :: "('a::linorder) set set" and leader :: "bal \<Rightarrow> ('a::linorder)" and next_bal as + 
+  fixes ampr3_ioa :: "(('a, 'v) global_state, 'v paxos_action) ioa" 
+    and ampr1_ioa :: "(('v, 'a, 'l) ampr1_state, 'v paxos_action) ioa" 
+  defines "ampr3_ioa \<equiv> ioa" and "ampr1_ioa \<equiv> r1.ioa"
+  fixes a1 a2 a3
+  assumes "a1 \<in> as" and "a2 \<in> as" and "a3 \<in> as" and "a1 \<noteq> a2" and "a3 \<noteq> a2" and "a3 \<noteq> a1"
+begin
+
+interpretation IOA .
+
+lemmas action_defs = propose_def do_2a_def receive_2b_def
+      try_acquire_leadership_def receive_1a_def receive_2a_def receive_1b_def receive_fwd_def
+lemmas init_defs = ampr3_ioa_def ioa_def global_start_def local_start_def
+  ampr1_ioa_def r1.ioa_def r1.start_def r1.start_s_def 
+
+method trans_cases =
+  (simp add:is_trans_def ampr3_ioa_def ioa_def, elim trans_cases)
+
+definition inv1 where inv1_def[inv_proofs_defs]:"inv1 s \<equiv> \<forall> a . acceptors (lstate s a) = as \<and> id (lstate s a) = a"
+lemma inv1:"invariant ampr3_ioa inv1"
+  apply (rule invariantI)
+   apply (simp add:inv1_def init_defs)
+  apply (rm_reachable)
+  apply trans_cases
+         apply (auto simp add:Let_def inv1_def action_defs)
+  done
+declare inv1[invs]
+
+fun extract_vs where 
+  "extract_vs (Fwd v) = {v}"
+| "extract_vs (Phase2a _ _ v) = {v}"
+| "extract_vs (Phase2b _ _ _ v) = {v}"
+| "extract_vs (Phase1b _ _ ff) = {v . \<exists> i b . ff $ i = Some (v,b)}"
+  -- {* Could be @{term "{ff $ i \<bind> (Some o fst) | i . True} \<bind> option_as_set" }*}
+| "extract_vs _ = {}"
+  
+definition propCmd where "propCmd s \<equiv> \<Union> ((\<lambda> p . case p of Packet _ m \<Rightarrow> extract_vs m) ` network s)"
+
+definition propCmd2 where "propCmd2 s \<equiv> {v . \<exists> a \<in> as . 
+  Packet a (Fwd v) \<in> network s 
+  \<or> (\<exists> i b . Packet a (Phase2a i b v) \<in> network s)
+  \<or> (\<exists> a2 \<in> as . \<exists> i b v . Packet a (Phase2b a2 i b v) \<in> network s)
+  \<or> (\<exists> a2 \<in> as . \<exists> b ff i b2 . Packet a (Phase1b a2 b ff) \<in> network s \<and> ff $ i = Some (v,b2))}"
+
+definition fwd_sim where "fwd_sim s \<equiv> {t . 
+  ampr1_state.propCmd t = propCmd s
+  \<and> ballot t = (\<lambda> a . acc.ballot (lstate s a))
+  \<and> (\<forall> i b v . suggestion t i b = None \<longleftrightarrow> (\<forall> a . Packet a (Phase2a i b v) \<notin> network s))
+  \<and> (\<forall> i b v . suggestion t i b = Some v \<longleftrightarrow> (\<forall> a . a \<noteq> leader b \<longrightarrow> Packet a (Phase2a i b v) \<in> network s))
+  \<and> (\<forall> i b v a . vote t i a b = None \<longleftrightarrow> (\<forall> a2 . Packet a2 (Phase2b a i b v) \<notin> network s))
+  \<and> (\<forall> i b v a . vote t i a b = Some v \<longleftrightarrow> (\<forall> a2 . a2 \<noteq> a \<longrightarrow> Packet a2 (Phase2b a i b v) \<in> network s))
+  \<and> (\<forall> a b ff . onebs t a b = None \<longleftrightarrow> (Packet (leader b) (Phase1b a b ff) \<notin> network s))
+  \<and> (\<forall> a b f . onebs t a b = Some f \<longleftrightarrow> (Packet (leader b) (Phase1b a b (Abs_finfun f)) \<in> network s))}"
+  
+lemmas sim_defs = fwd_sim_def propCmd_def 
+
+lemma "is_forward_sim fwd_sim ampr3_ioa ampr1_ioa"
+  apply (auto simp add:is_forward_sim_def)
+   apply (simp add:init_defs sim_defs)
+   apply (metis ref_proof_3.axioms(2) ref_proof_3_axioms ref_proof_3_axioms_def)
+  apply (insert invs)
+  apply (instantiate_invs)
+  apply (rm_reachable)
+  apply trans_cases
+  subgoal premises prems for s s' t act a v (* Propose *)
+  proof -
+    let ?ef = "[(act, s'\<lparr>ampr1_state.propCmd := insert v (ampr1_state.propCmd s')\<rparr>)]"
+    show ?thesis
+      apply (intro exI[where ?x="?ef"])
+      apply (intro conjI)
+        prefer 3
+        apply (force simp add:trace_match_def trace_def schedule_def externals_def
+          filter_act_def ampr1_ioa_def r1.ioa_def paxos_asig_def Let_def is_trans_def 
+          r1.trans_def split!:if_splits)
+       apply simp
+      subgoal proof (cases "leader (acc.ballot (lstate s a)) = acc.id (lstate s a)")
+        case False
+        with prems(1,4) show ?thesis by (simp add:propose_def send_all_def fwd_sim_def propCmd_def)
+      next
+        case True thm prems
+        have 1:"\<And> a . acc.ballot (lstate t a) = ballot s' a" using prems(1,4) True 
+          by (simp add:do_2a_def propose_def send_all_def fwd_sim_def Let_def propCmd_def)
+        have 2:"network t = network s \<union> {Packet a2 (Phase2a (next_inst (lstate s a)) (acc.ballot (lstate s a)) v) 
+            | a2 . a2 \<noteq> a \<and> a2 \<in> acceptors (lstate s a)}"
+          using prems(4,2) True
+          by (fastforce simp add:do_2a_def propose_def send_all_def fwd_sim_def propCmd_def Let_def inv1_def) oops
+        show ?thesis using 1 2 prems(1,2) apply (auto simp add:sim_defs inv1_def split!:msg.splits packet.splits)
+              apply (metis ref_proof_3.axioms(2) ref_proof_3_axioms ref_proof_3_axioms_def)
+             apply meson defer
+          apply meson oops
+end
+
+end
