Isabelle2/Utils.thy
@@ -1,0 +1,12 @@
+theory Utils
+imports Main
+begin
+
+definition option_as_set where "option_as_set x \<equiv> case x of None \<Rightarrow> {} | Some y \<Rightarrow> {y}"
+  
+abbreviation(input) flip where "flip f \<equiv> \<lambda> x y . f y x"
+  
+type_synonym bal = nat
+type_synonym inst = nat
+
+end
